Add a ring goal
Unfortunately, the ring proofs are a bit messy.

src/Experiments/SimplyTypedArithmetic.v
@@ -9,6 +9,7 @@ Require Import Crypto.Util.Tuple Crypto.Util.Prod Crypto.Util.LetIn.
 Require Import Crypto.Util.ListUtil Coq.Lists.List Crypto.Util.NatUtil.
 Require Import QArith.QArith_base QArith.Qround Crypto.Util.QUtil.
 Require Import Crypto.Algebra.Ring Crypto.Util.Decidable.Bool2Prop.
+Require Import Crypto.Util.ZUtil.Tactics.PullPush.Modulo.
 Require Import Crypto.Util.ZRange.
 Require Import Crypto.Util.ZRange.Operations.
 Require Import Crypto.Util.Tactics.RunTacticAsConstr.
@@ -16,13 +17,14 @@ Require Import Crypto.Util.Tactics.Head.
 Require Import Crypto.Util.Option.
 Require Import Crypto.Util.ZUtil.Tactics.LtbToLt.
 Require Import Crypto.Util.ZUtil.Tactics.PullPush.Modulo.
+Require Import Crypto.Util.Tactics.SpecializeBy.
 Require Import Crypto.Util.Notations.
 Require Import Crypto.Util.ZUtil.Definitions.
 Import ListNotations. Local Open Scope Z_scope.
 
 Module Associational.
   Definition eval (p:list (Z*Z)) : Z :=
-    fold_right Z.add 0%Z (map (fun t => fst t * snd t) p).
+    fold_right (fun x y => x + y) 0%Z (map (fun t => fst t * snd t) p).
 
   Lemma eval_nil : eval nil = 0.
   Proof. trivial.                                             Qed.
@@ -409,40 +411,116 @@ Module Positional. Section Positional.
   Hint Rewrite @eval_opp @eval_sub : push_eval.
   Hint Rewrite @length_sub @length_opp : distr_length.
 
-  Section carry_mulmod.
-    Context (s:Z)
-            (c:list (Z*Z))
+  Section mod_ops.
+    Context (s : Z)
+            (c : list (Z*Z))
             (n : nat)
             (len_c : nat)
             (idxs : list nat)
             (len_idxs : nat)
-            (fg : list Z * list Z).
+            (m_nz:s - Associational.eval c <> 0) (s_nz:s <> 0)
+            (Hn_nz : n <> 0%nat)
+            (Hc : length c = len_c)
+            (Hidxs : length idxs = len_idxs)
+            (Hw_div_nz : forall i : nat, weight (S i) / weight i <> 0).
 
     Derive carry_mulmod
-           SuchThat (forall (f := fst fg) (g := snd fg)
-                            (m_nz:s - Associational.eval c <> 0) (s_nz:s <> 0)
+           SuchThat (forall (fg : list Z * list Z)
+                            (f := fst fg) (g := snd fg)
                             (Hf : length f = n)
-                            (Hg : length g = n)
-                            (Hn_nz : n <> 0%nat)
-                            (Hc : length c = len_c)
-                            (Hidxs : length idxs = len_idxs)
-                            (Hw_div_nz : forall i : nat, weight (S i) / weight i <> 0),
-                        (eval n carry_mulmod) mod (s - Associational.eval c)
+                            (Hg : length g = n),
+                        (eval n (carry_mulmod fg)) mod (s - Associational.eval c)
                         = (eval n f * eval n g) mod (s - Associational.eval c))
            As eval_carry_mulmod.
     Proof.
       intros.
-      erewrite <-eval_mulmod with (s:=s) (c:=c)
-        by (subst; try assumption; try reflexivity).
+      rewrite <-eval_mulmod with (s:=s) (c:=c) by auto.
       etransitivity;
         [ | rewrite <- @eval_chained_carries with (s:=s) (c:=c) (idxs:=idxs)
-            by (subst; auto); reflexivity ].
+            by auto; reflexivity ].
       eapply f_equal2; [|trivial]. eapply f_equal.
       expand_lists ().
-      subst carry_mulmod.
-      reflexivity.
+      subst f g carry_mulmod; reflexivity.
     Qed.
-  End carry_mulmod.
+
+    Derive carrymod
+           SuchThat (forall (f : list Z)
+                            (Hf : length f = n),
+                        (eval n (carrymod f)) mod (s - Associational.eval c)
+                        = (eval n f) mod (s - Associational.eval c))
+           As eval_carrymod.
+    Proof.
+      intros.
+      etransitivity;
+        [ | rewrite <- @eval_chained_carries with (s:=s) (c:=c) (idxs:=idxs)
+            by auto; reflexivity ].
+      eapply f_equal2; [|trivial]. eapply f_equal.
+      expand_lists ().
+      subst carrymod; reflexivity.
+    Qed.
+
+    Derive addmod
+           SuchThat (forall (fg: list Z * list Z)
+                            (f := fst fg) (g := snd fg)
+                            (Hf : length f = n)
+                            (Hg : length g = n),
+                        (eval n (addmod fg)) mod (s - Associational.eval c)
+                        = (eval n f + eval n g) mod (s - Associational.eval c))
+           As eval_addmod.
+    Proof.
+      intros.
+      rewrite <-eval_add by assumption.
+      eapply f_equal2; [|trivial]. eapply f_equal.
+      expand_lists ().
+      subst f g addmod; reflexivity.
+    Qed.
+
+    Derive submod
+           SuchThat (forall (coef:Z)
+                            (fg: list Z * list Z)
+                            (f := fst fg) (g := snd fg)
+                            (Hf : length f = n)
+                            (Hg : length g = n),
+                        (eval n (submod coef fg)) mod (s - Associational.eval c)
+                        = (eval n f - eval n g) mod (s - Associational.eval c))
+           As eval_submod.
+    Proof.
+      intros.
+      rewrite <-eval_sub with (coef:=coef) by auto.
+      eapply f_equal2; [|trivial]. eapply f_equal.
+      expand_lists ().
+      subst f g submod; reflexivity.
+    Qed.
+
+    Derive oppmod
+           SuchThat (forall (coef:Z)
+                            (f: list Z)
+                            (Hf : length f = n),
+                        (eval n (oppmod coef f)) mod (s - Associational.eval c)
+                        = (- eval n f) mod (s - Associational.eval c))
+           As eval_oppmod.
+    Proof.
+      intros.
+      rewrite <-eval_opp with (coef:=coef) by auto.
+      eapply f_equal2; [|trivial]. eapply f_equal.
+      expand_lists ().
+      subst oppmod; reflexivity.
+    Qed.
+
+    Derive encodemod
+           SuchThat (forall (f:Z),
+                        (eval n (encodemod f)) mod (s - Associational.eval c)
+                        = f mod (s - Associational.eval c))
+           As eval_encodemod.
+    Proof.
+      intros.
+      etransitivity.
+      2:rewrite <-@eval_encode with (n:=n) by auto; reflexivity.
+      eapply f_equal2; [|trivial]. eapply f_equal.
+      expand_lists ().
+      subst encodemod; reflexivity.
+    Qed.
+  End mod_ops.
 End Positional. End Positional.
 
 Require Import Crypto.Util.ZUtil.AddGetCarry Crypto.Util.ZUtil.MulSplit.
@@ -1267,16 +1345,18 @@ Module Compilers.
                      do_reify_ident
                        term'
                        ltac:(fun _
-                             => let term
-                                    := match constr:(Set) with
-                                       | _ => (eval cbv delta [term] in term) (* might fail, so we wrap it in a match to give better error messages *)
-                                       | _
-                                         => let dummy := match goal with
-                                                         | _ => fail 2 "Unrecognized term:" term'
-                                                         end in
-                                            constr:(I : I)
-                                       end in
-                                reify_rec term)
+                             =>
+                               (*let __ := match goal with _ => idtac "Attempting to unfold" term end in*)
+                               let term
+                                   := match constr:(Set) with
+                                      | _ => (eval cbv delta [term] in term) (* might fail, so we wrap it in a match to give better error messages *)
+                                      | _
+                                        => let dummy := match goal with
+                                                        | _ => fail 2 "Unrecognized term:" term'
+                                                        end in
+                                           constr:(I : I)
+                                      end in
+                               reify_rec term)
                 end)
           end
         end.
@@ -1325,6 +1405,7 @@ Module Compilers.
           | Z_add : ident (Z * Z) Z
           | Z_mul : ident (Z * Z) Z
           | Z_pow : ident (Z * Z) Z
+          | Z_sub : ident (Z * Z) Z
           | Z_opp : ident Z Z
           | Z_div : ident (Z * Z) Z
           | Z_modulo : ident (Z * Z) Z
@@ -1390,6 +1471,7 @@ Module Compilers.
                | Z_pow => curry2 Z.pow
                | Z_modulo => curry2 Z.modulo
                | Z_opp => Z.opp
+               | Z_sub => curry2 Z.sub
                | Z_div => curry2 Z.div
                | Z_eqb => curry2 Z.eqb
                | Z_leb => curry2 Z.leb
@@ -1504,6 +1586,7 @@ Module Compilers.
             | Z.add ?x ?y => mkAppIdent ident.Z_add (x, y)
             | Z.mul ?x ?y => mkAppIdent ident.Z_mul (x, y)
             | Z.pow ?x ?y => mkAppIdent ident.Z_pow (x, y)
+            | Z.sub ?x ?y => mkAppIdent ident.Z_sub (x, y)
             | Z.opp ?x => mkAppIdent ident.Z_opp x
             | Z.div ?x ?y => mkAppIdent ident.Z_div (x, y)
             | Z.modulo ?x ?y => mkAppIdent ident.Z_modulo (x, y)
@@ -1549,6 +1632,7 @@ Module Compilers.
             Notation add := Z_add.
             Notation mul := Z_mul.
             Notation pow := Z_pow.
+            Notation sub := Z_sub.
             Notation opp := Z_opp.
             Notation div := Z_div.
             Notation modulo := Z_modulo.
@@ -1626,6 +1710,7 @@ Module Compilers.
           | Z_add : ident (Z * Z) Z
           | Z_mul : ident (Z * Z) Z
           | Z_pow : ident (Z * Z) Z
+          | Z_sub : ident (Z * Z) Z
           | Z_opp : ident Z Z
           | Z_div : ident (Z * Z) Z
           | Z_modulo : ident (Z * Z) Z
@@ -1685,6 +1770,7 @@ Module Compilers.
                | Z_mul => curry2 Z.mul
                | Z_pow => curry2 Z.pow
                | Z_modulo => curry2 Z.modulo
+               | Z_sub => curry2 Z.sub
                | Z_opp => Z.opp
                | Z_div => curry2 Z.div
                | Z_eqb => curry2 Z.eqb
@@ -1769,6 +1855,7 @@ Module Compilers.
             | Z.add ?x ?y => mkAppIdent ident.Z_add (x, y)
             | Z.mul ?x ?y => mkAppIdent ident.Z_mul (x, y)
             | Z.pow ?x ?y => mkAppIdent ident.Z_pow (x, y)
+            | Z.sub ?x ?y => mkAppIdent ident.Z_sub (x, y)
             | Z.opp ?x => mkAppIdent ident.Z_opp x
             | Z.div ?x ?y => mkAppIdent ident.Z_div (x, y)
             | Z.modulo ?x ?y => mkAppIdent ident.Z_modulo (x, y)
@@ -1807,6 +1894,7 @@ Module Compilers.
             Notation add := Z_add.
             Notation mul := Z_mul.
             Notation pow := Z_pow.
+            Notation sub := Z_sub.
             Notation opp := Z_opp.
             Notation div := Z_div.
             Notation modulo := Z_modulo.
@@ -1916,6 +2004,8 @@ Module Compilers.
                => AppIdent ident.Z.mul
              | for_reification.ident.Z_pow
                => AppIdent ident.Z.pow
+             | for_reification.ident.Z_sub
+               => AppIdent ident.Z.sub
              | for_reification.ident.Z_opp
                => AppIdent ident.Z.opp
              | for_reification.ident.Z_div
@@ -2205,6 +2295,15 @@ Module Compilers.
               | ident.primitive _ v => Some v
               | _ => None
               end
+         | None => None
+         end.
+    Definition invert_Z_opp (e : @expr var type.Z) : option (@expr var type.Z)
+      := match invert_AppIdent e with
+         | Some (existT s (idc, args))
+           => match idc in ident s t return expr s -> option (expr type.Z) with
+              | ident.Z_opp => fun v => Some v
+              | _ => fun _ => None
+              end args
          | None => None
          end.
 
@@ -2710,6 +2809,7 @@ Module Compilers.
                   | ident.Z_add as idc
                   | ident.Z_mul as idc
                   | ident.Z_pow as idc
+                  | ident.Z_sub as idc
                   | ident.Z_opp as idc
                   | ident.Z_div as idc
                   | ident.Z_modulo as idc
@@ -2905,6 +3005,7 @@ Module Compilers.
                             @@ (ident.fst @@ (Var xyk)))
                 | ident.Z_add as idc
                 | ident.Z_mul as idc
+                | ident.Z_sub as idc
                 | ident.Z_pow as idc
                 | ident.Z_div as idc
                 | ident.Z_modulo as idc
@@ -3321,6 +3422,36 @@ Module Compilers.
     Include default.
   End CPS.
 
+  Module sign.
+    Local Set Boolean Equality Schemes.
+    Local Set Decidable Equality Schemes.
+    Inductive sign := pos | neg.
+    Module Z.
+      Definition interp (s : sign) : Z -> Z
+        := match s with
+           | pos => id
+           | neg => Z.opp
+           end.
+    End Z.
+    Definition of_Z (v : Z) : sign
+      := match v with
+         | Zneg _ => neg
+         | Zpos _ => pos
+         | Z0 => (* default *) pos
+         end.
+    Definition opp (s : sign) : sign
+      := match s with
+         | pos => neg
+         | neg => pos
+         end.
+    Definition mul (s1 s2 : sign) : sign
+      := match s1, s2 with
+         | pos, pos => pos
+         | neg, neg => pos
+         | pos, neg | neg, pos => neg
+         end.
+  End sign.
+  Notation sign := sign.sign.
   Module partial.
     Section value.
       Context (var : type -> Type).
@@ -3336,6 +3467,8 @@ Module Compilers.
         := match t return Type with
            | type.arrow _ _ as t
              => value_prestep value t
+           | type.type_primitive type.Z as t
+             => sign * @expr var t + value_prestep value t
            | type.prod _ _ as t
            | type.list _ as t
            | type.type_primitive _ as t
@@ -3367,6 +3500,13 @@ Module Compilers.
                      | inl v => v
                      | inr v => reify_list (List.map (@reify A) v)
                      end
+             | type.type_primitive type.Z as t
+               => fun x : sign * expr t + type.interp t
+                  => match x with
+                     | inl (sign.pos, v) => v
+                     | inl (sign.neg, v) => ident.Z.opp @@ v
+                     | inr v => ident.primitive v @@ TT
+                     end%core%expr
              | type.type_primitive _ as t
                => fun x : expr t + type.interp t
                   => match x with
@@ -3399,6 +3539,15 @@ Module Compilers.
                           => inr (List.map (@reflect A) ls)
                         | None
                           => inl v
+                        end
+                | type.type_primitive type.Z as t
+                  => fun v : expr t
+                     => let inr := @inr (sign * expr t) (value_prestep (value var) t) in
+                        let inl := @inl (sign * expr t) (value_prestep (value var) t) in
+                        match reflect_primitive v, invert_Z_opp v with
+                        | Some v, _ => inr v
+                        | None, Some v => inl (sign.neg, v)
+                        | None, None => inl (sign.pos, v)
                         end
                 | type.type_primitive _ as t
                   => fun v : expr t
@@ -3446,6 +3595,17 @@ Module Compilers.
                                   (fun b => f (inr (a, b))))
                      | inl e => partial.expr.reflect (expr_let y := e in partial.expr.reify (f (inl (Var y))))%expr
                      end
+             | type.type_primitive type.Z as t
+               => fun (x : sign * expr t + type.interp t)
+                      (f : sign * expr t + type.interp t -> value var tC)
+                  => match x with
+                     | inl (sgn, e)
+                       => match invert_Var e with
+                          | Some v => f (inl (sgn, Var v))
+                          | None => partial.expr.reflect (expr_let y := e in partial.expr.reify (f (inl (sgn, Var y)%core)))%expr
+                          end
+                     | inr v => f (inr v)
+                     end
              | type.type_primitive _ as t
                => fun (x : expr t + type.interp t) (f : expr t + type.interp t -> value var tC)
                   => match x with
@@ -3468,6 +3628,8 @@ Module Compilers.
                      end
              | ident.nil t
                => fun _ => inr (@nil (value var t))
+             | ident.primitive type.Z v
+               => fun _ => inr v
              | ident.primitive t v
                => fun _ => inr v
              | ident.cons t as idc
@@ -3517,6 +3679,15 @@ Module Compilers.
                             ls
                      | _ => expr.reflect (AppIdent idc (expr.reify (t:=P * (A * type.list A * P -> P) * type.list A) nil_case_cons_case_ls))
                      end
+             | ident.List.nth_default type.Z as idc
+               => fun (default_ls_idx : expr (type.Z * type.list type.Z * type.nat) + (expr (type.Z * type.list type.Z) + (sign * expr type.Z + type.interp type.Z) * (expr (type.list type.Z) + list (value var type.Z))) * (expr type.nat + nat))
+                  => match default_ls_idx with
+                     | inr (inr (default, inr ls), inr idx)
+                       => List.nth_default default ls idx
+                     | inr (inr (inr default, ls), inr idx)
+                       => expr.reflect (AppIdent (ident.List.nth_default_concrete default idx) (expr.reify (t:=type.list type.Z) ls))
+                     | _ => expr.reflect (AppIdent idc (expr.reify (t:=type.Z * type.list type.Z * type.nat) default_ls_idx))
+                     end
              | ident.List.nth_default (type.type_primitive A) as idc
                => fun (default_ls_idx : expr (A * type.list A * type.nat) + (expr (A * type.list A) + (expr A + type.interp A) * (expr (type.list A) + list (value var A))) * (expr type.nat + nat))
                   => match default_ls_idx with
@@ -3542,8 +3713,8 @@ Module Compilers.
                      end
              | ident.Z_mul_split as idc
                => fun (x_y_z :  (expr (type.Z * type.Z * type.Z) +
-                                 (expr (type.Z * type.Z) + (expr type.Z + Z) * (expr type.Z + Z)) * (expr type.Z + Z))%type)
-                  => match x_y_z return (expr _ + (expr _ + type.interp _) * (expr _ + type.interp _)) with
+                                 (expr (type.Z * type.Z) + (sign * expr type.Z + Z) * (sign * expr type.Z + Z)) * (sign * expr type.Z + Z))%type)
+                  => match x_y_z return (expr _ + (sign * expr _ + type.interp _) * (sign * expr _ + type.interp _)) with
                      | inr (inr (inr x, inr y), inr z) =>
                        let result := ident.interp idc (x, y, z) in
                        inr (inr (fst result), inr (snd result))
@@ -3553,8 +3724,8 @@ Module Compilers.
                      end
              | ident.Z_add_get_carry as idc
                => fun (x_y_z :  (expr (type.Z * type.Z * type.Z) +
-                                 (expr (type.Z * type.Z) + (expr type.Z + Z) * (expr type.Z + Z)) * (expr type.Z + Z))%type)
-                  => match x_y_z return (expr _ + (expr _ + type.interp _) * (expr _ + type.interp _)) with
+                                 (expr (type.Z * type.Z) + (sign * expr type.Z + Z) * (sign * expr type.Z + Z)) * (sign * expr type.Z + Z))%type)
+                  => match x_y_z return (expr _ + (sign * expr _ + type.interp _) * (sign * expr _ + type.interp _)) with
                      | inr (inr (inr x, inr y), inr z) =>
                        let result := ident.interp idc (x, y, z) in
                        inr (inr (fst result), inr (snd result))
@@ -3573,9 +3744,9 @@ Module Compilers.
              | ident.Z_add_with_get_carry as idc
                => fun (x_y_z_a : (expr (_ * _ * _ * _) +
                                   (expr (_ * _ * _) +
-                                   (expr (_ * _) + (expr _ + type.interp _) * (expr _ + type.interp _)) *
-                                   (expr _ + type.interp _)) * (expr _ + type.interp _))%type)
-                  => match x_y_z_a return (expr _ + (expr _ + type.interp _) * (expr _ + type.interp _)) with
+                                   (expr (_ * _) + (sign * expr _ + type.interp _) * (sign * expr _ + type.interp _)) *
+                                   (sign * expr _ + type.interp _)) * (sign * expr _ + type.interp _))%type)
+                  => match x_y_z_a return (expr _ + (sign * expr _ + type.interp _) * (sign * expr _ + type.interp _)) with
                      | inr (inr (inr (inr x, inr y), inr z), inr a) =>
                        let result := ident.interp idc (x, y, z, a) in
                        inr (inr (fst result), inr (snd result))
@@ -3585,8 +3756,8 @@ Module Compilers.
                      end
              | ident.Z_sub_get_borrow as idc
                => fun (x_y_z :  (expr (type.Z * type.Z * type.Z) +
-                                 (expr (type.Z * type.Z) + (expr type.Z + Z) * (expr type.Z + Z)) * (expr type.Z + Z))%type)
-                  => match x_y_z return (expr _ + (expr _ + type.interp _) * (expr _ + type.interp _)) with
+                                 (expr (type.Z * type.Z) + (sign * expr type.Z + Z) * (sign * expr type.Z + Z)) * (sign * expr type.Z + Z))%type)
+                  => match x_y_z return (expr _ + (sign * expr _ + type.interp _) * (sign * expr _ + type.interp _)) with
                      | inr (inr (inr x, inr y), inr z) =>
                        let result := ident.interp idc (x, y, z) in
                        inr (inr (fst result), inr (snd result))
@@ -3596,17 +3767,17 @@ Module Compilers.
                      end
              | ident.Z_mul_split_concrete _ as idc
              | ident.Z.sub_get_borrow_concrete _ as idc
-               => fun (x_y : expr (_ * _) + (expr _ + type.interp _) * (expr _ + type.interp _))
-                  => match x_y return (expr _ + (expr _ + type.interp _) * (expr _ + type.interp _)) with
+               => fun (x_y : expr (_ * _) + (sign * expr _ + type.interp _) * (sign * expr _ + type.interp _))
+                  => match x_y return (expr _ + (sign * expr _ + type.interp _) * (sign * expr _ + type.interp _)) with
                      | inr (inr x, inr y) =>
                        let result := ident.interp idc (x, y) in
                        inr (inr (fst result), inr (snd result))
                      | _ => expr.reflect (AppIdent idc (expr.reify (t:=_*_) x_y))
                      end
              | ident.Z.add_get_carry_concrete _ as idc
-               => fun (x_y : expr (_ * _) + (expr _ + type.interp _) * (expr _ + type.interp _))
+               => fun (x_y : expr (_ * _) + (sign * expr _ + type.interp _) * (sign * expr _ + type.interp _))
                   => let default := expr.reflect (AppIdent idc (expr.reify (t:=_*_) x_y)) in
-                     match x_y return (expr _ + (expr _ + type.interp _) * (expr _ + type.interp _)) with
+                     match x_y return (expr _ + (sign * expr _ + type.interp _) * (sign * expr _ + type.interp _)) with
                      | inr (inr x, inr y) =>
                        let result := ident.interp idc (x, y) in
                        inr (inr (fst result), inr (snd result))
@@ -3619,8 +3790,8 @@ Module Compilers.
                      end
              | ident.Z.add_with_get_carry_concrete _ as idc
                => fun (x_y_z :  (expr (type.Z * type.Z * type.Z) +
-                                 (expr (type.Z * type.Z) + (expr type.Z + Z) * (expr type.Z + Z)) * (expr type.Z + Z))%type)
-                  => match x_y_z return (expr _ + (expr _ + type.interp _) * (expr _ + type.interp _)) with
+                                 (expr (type.Z * type.Z) + (sign * expr type.Z + Z) * (sign * expr type.Z + Z)) * (sign * expr type.Z + Z))%type)
+                  => match x_y_z return (expr _ + (sign * expr _ + type.interp _) * (sign * expr _ + type.interp _)) with
                      | inr (inr (inr x, inr y), inr z) =>
                        let result := ident.interp idc (x, y, z) in
                        inr (inr (fst result), inr (snd result))
@@ -3628,30 +3799,50 @@ Module Compilers.
                      end
              | ident.pred as idc
              | ident.Nat_succ as idc
-             | ident.Z_of_nat as idc
-             | ident.Z_opp as idc
-             | ident.Z_shiftr _ as idc
-             | ident.Z_shiftl _ as idc
-             | ident.Z_land _ as idc
                => fun x : expr _ + type.interp _
                   => match x return expr _ + type.interp _ with
                      | inr x => inr (ident.interp idc x)
                      | inl x => expr.reflect (AppIdent idc x)
                      end
+             | ident.Z_of_nat as idc
+               => fun x : expr _ + type.interp _
+                  => match x return sign * expr _ + type.interp _ with
+                     | inr x => inr (ident.interp idc x)
+                     | inl x => expr.reflect (AppIdent idc x)
+                     end
+             | ident.Z_opp as idc
+               => fun x : sign * expr _ + type.interp _
+                  => match x return sign * expr _ + type.interp _ with
+                     | inr x => inr (ident.interp idc x)
+                     | inl (sgn, x) => inl (sign.opp sgn, x)
+                     end
+             | ident.Z_shiftr _ as idc
+             | ident.Z_shiftl _ as idc
+             | ident.Z_land _ as idc
+               => fun x : sign * expr _ + type.interp _
+                  => match x return sign * expr _ + type.interp _ with
+                     | inr x => inr (ident.interp idc x)
+                     | inl _ => expr.reflect (AppIdent idc (expr.reify (t:=type.Z) x))
+                     end
              | ident.Nat_add as idc
              | ident.Nat_mul as idc
              | ident.Z_pow as idc
+               => fun (x_y : expr (_ * _) + (sign * expr _ + type.interp _) * (sign * expr _ + type.interp _))
+                  => match x_y return sign * expr _ + type.interp _ with
+                     | inr (inr x, inr y) => inr (ident.interp idc (x, y))
+                     | _ => expr.reflect (AppIdent idc (expr.reify (t:=_*_) x_y))
+                     end
              | ident.Z_eqb as idc
              | ident.Z_leb as idc
-               => fun (x_y : expr (_ * _) + (expr _ + type.interp _) * (expr _ + type.interp _))
+               => fun (x_y : expr (_ * _) + (sign * expr _ + type.interp _) * (sign * expr _ + type.interp _))
                   => match x_y return expr _ + type.interp _ with
                      | inr (inr x, inr y) => inr (ident.interp idc (x, y))
                      | _ => expr.reflect (AppIdent idc (expr.reify (t:=_*_) x_y))
                      end
              | ident.Z_div as idc
-               => fun (x_y : expr (_ * _) + (expr _ + type.interp _) * (expr _ + type.interp _))
+               => fun (x_y : expr (_ * _) + (sign * expr _ + type.interp _) * (sign * expr _ + type.interp _))
                   => let default := expr.reflect (AppIdent idc (expr.reify (t:=_*_) x_y)) in
-                     match x_y return expr _ + type.interp _ with
+                     match x_y return sign * expr _ + type.interp _ with
                      | inr (inr x, inr y) => inr (ident.interp idc (x, y))
                      | inr (x, inr y)
                        => if Z.eqb y (2^Z.log2 y)
@@ -3660,9 +3851,9 @@ Module Compilers.
                      | _ => default
                      end
              | ident.Z_modulo as idc
-               => fun (x_y : expr (_ * _) + (expr _ + type.interp _) * (expr _ + type.interp _))
+               => fun (x_y : expr (_ * _) + (sign * expr _ + type.interp _) * (sign * expr _ + type.interp _))
                   => let default := expr.reflect (AppIdent idc (expr.reify (t:=_*_) x_y)) in
-                     match x_y return expr _ + type.interp _ with
+                     match x_y return sign * expr _ + type.interp _ with
                      | inr (inr x, inr y) => inr (ident.interp idc (x, y))
                      | inr (x, inr y)
                        => if Z.eqb y (2^Z.log2 y)
@@ -3671,38 +3862,82 @@ Module Compilers.
                      | _ => default
                      end
              | ident.Z_mul as idc
-               => fun (x_y : expr (_ * _) + (expr _ + type.interp _) * (expr _ + type.interp _))
+               => fun (x_y : expr (_ * _) + (sign * expr _ + type.interp _) * (sign * expr _ + type.interp _))
                   => let default := expr.reflect (AppIdent idc (expr.reify (t:=_*_) x_y)) in
-                     match x_y return expr _ + type.interp _ with
+                     match x_y return sign * expr _ + type.interp _ with
                      | inr (inr x, inr y) => inr (ident.interp idc (x, y))
-                     | inr (inr x, inl e)
-                     | inr (inl e, inr x)
+                     | inr (inr x, inl (sgn, e))
+                     | inr (inl (sgn, e), inr x)
                        => if Z.eqb x 0
                           then inr 0%Z
                           else if Z.eqb x 1
-                               then inl e
-                               else if Z.eqb x (2^Z.log2 x)
-                                    then expr.reflect (AppIdent (ident.Z.shiftl (Z.log2 x)) e)
-                                    else default
-                     | inr (inl _, inl _) | inl _ => default
+                               then inl (sgn, e)
+                               else if Z.eqb x (-1)
+                                    then inl (sign.opp sgn, e)
+                                    else let sgn' := sign.mul sgn (sign.of_Z x) in
+                                         let x' := Z.abs x in
+                                         if Z.eqb x' (2^Z.log2 x')
+                                         then inl (sgn',
+                                                   AppIdent (ident.Z.shiftl (Z.log2 x')) e)
+                                         else inl (sgn',
+                                                   AppIdent idc (ident.primitive (t:=type.Z) x @@ TT, e))
+                     | inr (inl (sgna, a), inl (sgnb, b))
+                       => inl (sign.mul sgna sgnb, AppIdent idc (a, b))
+                     | inl _ => default
                      end
              | ident.Z_add as idc
-               => fun (x_y : expr (_ * _) + (expr _ + type.interp _) * (expr _ + type.interp _))
+               => fun (x_y : expr (_ * _) + (sign * expr _ + type.interp _) * (sign * expr _ + type.interp _))
                   => let default := expr.reflect (AppIdent idc (expr.reify (t:=_*_) x_y)) in
-                     match x_y return expr _ + type.interp _ with
+                     match x_y return sign * expr _ + type.interp _ with
                      | inr (inr x, inr y) => inr (ident.interp idc (x, y))
-                     | inr (inr x, inl e)
-                     | inr (inl e, inr x)
+                     | inr (inr x, inl (sgn, e))
+                     | inr (inl (sgn, e), inr x)
                        => if Z.eqb x 0
-                          then inl e
+                          then inl (sgn, e)
+                          else match sgn with
+                               | sign.pos => default
+                               | sign.neg
+                                 => inl (sign.pos,
+                                         AppIdent
+                                           ident.Z.sub
+                                           (ident.primitive (t:=type.Z) x @@ TT,
+                                            e))
+                               end
+                     | inr (inl (sign.pos, p), inl (sign.neg, n))
+                     | inr (inl (sign.neg, n), inl (sign.pos, p))
+                       => inl (sign.pos, AppIdent ident.Z.sub (p, n)%expr)
+                     | inr (inl (sign.neg, a), inl (sign.neg, b))
+                       => inl (sign.neg, AppIdent idc (a, b)%expr)
+                     | inr (inl (sign.pos, _), inl (sign.pos, _))
+                     | inl _ => default
+                     end
+             | ident.Z_sub as idc
+               => fun (x_y : expr (_ * _) + (sign * expr _ + type.interp _) * (sign * expr _ + type.interp _))
+                  => let default := expr.reflect (AppIdent idc (expr.reify (t:=_*_) x_y)) in
+                     match x_y return sign * expr _ + type.interp _ with
+                     | inr (inr x, inr y) => inr (ident.interp idc (x, y))
+                     | inr (inr x, inl (sgn, e))
+                       => if Z.eqb x 0
+                          then inl (sign.opp sgn, e)
                           else default
-                     | inr (inl _, inl _) | inl _ => default
+                     | inr (inl (sgn, e), inr x)
+                       => if Z.eqb x 0
+                          then inl (sgn, e)
+                          else default
+                     | inr (inl (sign.pos, p), inl (sign.neg, n))
+                       => inl (sign.pos, AppIdent ident.Z.add (p, n))
+                     | inr (inl (sign.neg, n), inl (sign.pos, p))
+                       => inl (sign.neg, AppIdent ident.Z.add (p, n))
+                     | inr (inl (sign.neg, a), inl (sign.neg, b))
+                       => inl (sign.pos, AppIdent ident.Z.sub (b, a))
+                     | inr (inl (sign.pos, _), inl (sign.pos, _))
+                     | inl _ => default
                      end
              | ident.Z_zselect as idc
              | ident.Z_add_modulo as idc
                => fun (x_y_z :  (expr (_ * _ * _) +
-                                 (expr (_ * _) + (expr _ + type.interp _) * (expr _ + type.interp _)) * (expr _ + type.interp _))%type)
-                  => match x_y_z return expr _ + type.interp _ with
+                                 (expr (_ * _) + (sign * expr _ + type.interp _) * (sign * expr _ + type.interp _)) * (sign * expr _ + type.interp _))%type)
+                  => match x_y_z return sign * expr _ + type.interp _ with
                      | inr (inr (inr x, inr y), inr z) => inr (ident.interp idc (x, y, z))
                      | _ => expr.reflect (AppIdent idc (expr.reify (t:=_*_*_) x_y_z))
                      end
@@ -3941,6 +4176,7 @@ Module Compilers.
       | List_nth {T : type.primitive} (n : nat) : ident (list T) T
       | mul (T1 T2 Tout : type.primitive) : ident (T1 * T2) Tout
       | add (T1 T2 Tout : type.primitive) : ident (T1 * T2) Tout
+      | sub (T1 T2 Tout : type.primitive) : ident (T1 * T2) Tout
       | shiftr (T1 Tout : type.primitive) (offset : BinInt.Z) : ident T1 Tout
       | shiftl (T1 Tout : type.primitive) (offset : BinInt.Z) : ident T1 Tout
       | land (T1 Tout : type.primitive) (mask : BinInt.Z) : ident T1 Tout
@@ -3960,7 +4196,8 @@ Module Compilers.
       Notation curry3 f
         := (fun '(a, b, c) => f a b c).
 
-      Axiom admit : forall {T}, T.
+      Axiom admit_pf : False.
+      Notation admit := (match admit_pf with end).
 
       Definition resize {T1 Tout : type.primitive} : type.interp T1 -> type.interp Tout
         := match T1, Tout return type.interp T1 -> type.interp Tout with
@@ -4021,6 +4258,7 @@ Module Compilers.
            | snd A B => @Datatypes.snd (type.interp A) (type.interp B)
            | List_nth T n => fun ls => @List.nth_default (type.interp T) default ls n
            | add T1 T2 Tout => @resize2uc type.Z type.Z type.Z _ _ _ (curry2 Z.add)
+           | sub T1 T2 Tout => @resize2uc type.Z type.Z type.Z _ _ _ (curry2 Z.sub)
            | mul T1 T2 Tout => @resize2uc type.Z type.Z type.Z _ _ _ (curry2 Z.mul)
            | shiftr _ _ n => @resize1 type.Z type.Z _ _ (fun v => Z.shiftr v n)
            | shiftl _ _ n => @resize1 type.Z type.Z _ _ (fun v => Z.shiftl v n)
@@ -4041,6 +4279,7 @@ Module Compilers.
 
       Module Z.
         Notation mul := (@mul type.Z type.Z type.Z).
+        Notation sub := (@sub type.Z type.Z type.Z).
         Notation add := (@add type.Z type.Z type.Z).
         Notation shiftr := (@shiftr type.Z type.Z).
         Notation shiftl := (@shiftl type.Z type.Z).
@@ -4101,6 +4340,44 @@ Module Compilers.
                        else false
                end.
 
+          Definition primitive_bounded_by {t} : type.primitive.interp t -> zrange -> bool
+            := match t return primitive.interp t -> zrange -> bool with
+               | unit => fun _ _ => true
+               | Z => fun v r => (lower r <=? v) && (v <=? upper r)
+               | ZBounded _ _
+                 => fun v r => (lower r <=? value v) && (value v <=? upper r)
+               end.
+
+          Fixpoint list_bounded_by {t} (ls : Datatypes.list (primitive.interp t))
+                   (r : Datatypes.list zrange)
+            : bool
+            := match ls, r with
+               | nil, nil => true
+               | nil, _ => false
+               | cons x xs, cons r rs
+                 => primitive_bounded_by x r && @list_bounded_by _ xs rs
+               | cons _ _, _ => false
+               end.
+
+          Lemma length_list_bounded_by {t} ls r
+                (H : @list_bounded_by t ls r = true)
+            : List.length ls = List.length r.
+          Proof.
+            revert dependent r; induction ls as [|x xs IHxs], r;
+              cbn; try reflexivity; try discriminate.
+            rewrite Bool.andb_true_iff.
+            intros [? ?]; erewrite IHxs; [ reflexivity | assumption ].
+          Qed.
+
+          Fixpoint bounded_by {t} : type.interp t -> range t -> bool
+            := match t return type.interp t -> range t -> bool with
+               | type_primitive x => primitive_bounded_by
+               | prod A B => fun '((a, a') : type.interp A * type.interp B)
+                                 '((r, r') : range A * range B)
+                             => @bounded_by A a r && @bounded_by B a' r'
+               | list A => list_bounded_by
+               end.
+
           Fixpoint type_for_range {t} : range t -> type
             := match t return range t -> type with
                | type_primitive _ => primitive_for_zrange
@@ -4111,6 +4388,18 @@ Module Compilers.
                  => fun ls : Datatypes.list zrange
                     => type.list
                          (primitive_for_zrange (List.fold_right ZRange.union r[0 ~> 0]%zrange ls))
+               end.
+
+          Fixpoint type_for_range_bounded_by {t}
+            : forall (r : range t)
+                     (v : type.interp (type_for_range r)),
+              bool
+            := match t return forall (r : range t), type.interp (type_for_range r) -> bool with
+               | type_primitive x => fun r v => primitive_bounded_by v r
+               | prod A B => fun '((r, r') : range A * range B)
+                                 '((a, a') : type.interp (type_for_range r) * type.interp (type_for_range r'))
+                             => @type_for_range_bounded_by A r a && @type_for_range_bounded_by B r' a'
+               | list A => fun r v => list_bounded_by v r
                end.
         End with_relax.
       End Range.
@@ -4245,6 +4534,8 @@ Module Compilers.
                  => Some Z.mul
                | default.ident.Z_add
                  => Some Z.add
+               | default.ident.Z_sub
+                 => Some Z.sub
                | ident.Z_shiftr n
                  => Some (Z.shiftr n)
                | ident.Z_shiftl n
@@ -4373,18 +4664,7 @@ Module Compilers.
           Context (relax_zrange : zrange -> option zrange).
 
           Local Notation primitive_for_zrange := (primitive_for_zrange relax_zrange).
-
-          Fixpoint type_for_range {t} : range t -> type
-            := match t return range t -> type with
-               | type_primitive _ => primitive_for_zrange
-               | prod A B => fun (ab : range A * range B)
-                             => prod (@type_for_range A (Datatypes.fst ab))
-                                     (@type_for_range B (Datatypes.snd ab))
-               | list A
-                 => fun ls : Datatypes.list zrange
-                    => type.list
-                         (primitive_for_zrange (List.fold_right ZRange.union r[0 ~> 0]%zrange ls))
-               end.
+          Local Notation type_for_range := (type_for_range relax_zrange).
 
           Definition upper_lor_and_bounds (x y : BinInt.Z) : BinInt.Z
             := 2^(1 + Z.log2_up (Z.max x y)).
@@ -4582,6 +4862,11 @@ Module Compilers.
                       (fun '(existT r args)
 		       => existT _ (ZRange.four_corners BinInt.Z.add (Datatypes.fst r) (Datatypes.snd r))
                                  (AppIdent (add _ _ _) args))
+               | sub _ _ _
+                 => option_map
+                      (fun '(existT r args)
+		       => existT _ (ZRange.four_corners BinInt.Z.sub (Datatypes.fst r) (Datatypes.snd r))
+                                 (AppIdent (sub _ _ _) args))
                | shiftr _ _ offset
                  => option_map
                       (fun '(existT r args)
@@ -4696,7 +4981,7 @@ Module Compilers.
                  (s_bounds : range (Indexed.OfPHOAS.type.compile s))
       : option
           { bs : range (Indexed.OfPHOAS.type.compile d) &
-                 @expr ident (AdjustBounds.ident.type_for_range relax_zrange bs) }
+                 @expr ident (type_for_range relax_zrange bs) }
         := let e := Indexed.OfPHOAS.expr.Compile e in
            match e with
            | Some e
@@ -4729,12 +5014,12 @@ Module Compilers.
                  {d : Compilers.type.Notations.type}
                  (relax_zrange : zrange -> option zrange)
                  {bs : range (Indexed.OfPHOAS.type.compile d)}
-                 (v : type.interp (AdjustBounds.ident.type_for_range relax_zrange bs))
+                 (v : type.interp (type_for_range relax_zrange bs))
                  {struct d}
         : Compilers.type.interp d
         := match d
                  return (forall bs : range (Indexed.OfPHOAS.type.compile d),
-                            type.interp (AdjustBounds.ident.type_for_range relax_zrange bs)
+                            type.interp (type_for_range relax_zrange bs)
                             -> Compilers.type.interp d)
            with
            | Compilers.type.type_primitive x => @cast_back_primitive _ _
@@ -4742,7 +5027,7 @@ Module Compilers.
              => fun (bs :
                        (* ignore this line, for type inference badness *) range (Indexed.OfPHOAS.type.compile A) * range (Indexed.OfPHOAS.type.compile B))
                     (v :
-                       (* ignore this line, for type inference badness *) type.interp (AdjustBounds.ident.type_for_range relax_zrange (fst bs)) * type.interp (AdjustBounds.ident.type_for_range relax_zrange (snd bs)))
+                       (* ignore this line, for type inference badness *) type.interp (type_for_range relax_zrange (fst bs)) * type.interp (type_for_range relax_zrange (snd bs)))
                 => (@cast_back A relax_zrange (fst bs) (fst v),
                     @cast_back B relax_zrange (snd bs) (snd v))
            | type.arrow s d => fun bs v _ => @cast_back d relax_zrange bs v
@@ -4752,17 +5037,93 @@ Module Compilers.
            | Compilers.type.list A => fun _ _ => nil
            end bs v.
 
+      Definition option_cast_back
+                 {d : Compilers.type.Notations.type}
+                 (relax_zrange : zrange -> option zrange)
+                 {bs : range (Indexed.OfPHOAS.type.compile d)}
+                 (v : option (type.interp (type_for_range relax_zrange bs)))
+        := option_map (@cast_back d relax_zrange bs) v.
+
+      Definition relax_is_good
+                 (relax_zrange : zrange -> option zrange)
+        : Prop
+        := forall z z', relax_zrange z = Some z'
+                        -> is_tighter_than_bool z z' = true.
+
+      Definition cast_primitiveZ
+                 (d : Compilers.type.primitive := Compilers.type.Z)
+                 (relax_zrange : zrange -> option zrange)
+                 {bs : zrange}
+                 (v : Compilers.type.interp d)
+                 (Hrelax : relax_is_good relax_zrange)
+                 (Hv : is_bounded_by' None bs v)
+        : type.primitive.interp (primitive_for_zrange relax_zrange bs).
+      Proof.
+        cbn in *; hnf in Hv; cbv [primitive_for_zrange primitive_for_option_zrange].
+        specialize (Hrelax bs).
+        destruct (relax_zrange bs) as [bs'|]; [ exists v | exact v ].
+        clear d relax_zrange.
+        abstract (
+            specialize (Hrelax bs' eq_refl);
+            unfold is_tighter_than_bool in *;
+            rewrite Bool.andb_true_iff in *; split;
+            destruct_head'_and;
+            Z.ltb_to_lt;
+            (apply Z.min_case_strong || apply Z.max_case_strong);
+            omega
+          ).
+      Defined.
+
+      Lemma cast_back_primitive_cast_primitive
+            relax_zrange bs v Hrelax Hv
+        : cast_back_primitive relax_zrange
+                              (@cast_primitiveZ relax_zrange bs v Hrelax Hv)
+          = v.
+      Proof.
+        cbv [cast_primitiveZ]; cbn.
+        generalize (Hrelax bs).
+        break_innermost_match; reflexivity.
+      Qed.
+
       Definition Interp
                  {s d : Compilers.type.Notations.type}
                  (relax_zrange : zrange -> option zrange)
                  (s_bounds : range (Indexed.OfPHOAS.type.compile s))
                  {bs : range (Indexed.OfPHOAS.type.compile d)}
-                 (args : type.interp (AdjustBounds.ident.type_for_range relax_zrange s_bounds))
-                 (e : @expr ident (AdjustBounds.ident.type_for_range relax_zrange bs))
+                 (args : type.interp (type_for_range relax_zrange s_bounds))
+                 (e : @expr ident (type_for_range relax_zrange bs))
         : option (Compilers.type.interp d)
         := let ctx := extendb (PositiveMap.empty _) 1 args in
            let v := Indexed.expr.interp (@ident.interp) e ctx in
-           option_map (cast_back relax_zrange) v.
+           option_cast_back relax_zrange v.
+
+      Definition AnalyzeBoundsConst
+                 {d : Compilers.type.Notations.type}
+                 (relax_zrange : zrange -> option zrange)
+                 (e : Expr d)
+        : option
+            { bs : range (Indexed.OfPHOAS.type.compile d) &
+                   @expr ident (type_for_range relax_zrange bs) }
+        := let e := Indexed.OfPHOAS.expr.Compile e in
+           match e with
+           | Some e
+             => let e := AdjustBounds.expr.adjust_bounds
+                           relax_zrange
+                           (PositiveMap.empty _)
+                           e in
+                e
+           | None => None
+           end.
+
+      Definition InterpConst
+                 {d : Compilers.type.Notations.type}
+                 (relax_zrange : zrange -> option zrange)
+                 {bs : range (Indexed.OfPHOAS.type.compile d)}
+                 (e : @expr ident (type_for_range relax_zrange bs))
+        : option (Compilers.type.interp d)
+        := let ctx := PositiveMap.empty _ in
+           let v := Indexed.expr.interp (@ident.interp) e ctx in
+           option_cast_back relax_zrange v.
     End OfPHOAS.
   End BoundsAnalysis.
 End Compilers.
@@ -4962,7 +5323,33 @@ Module test6.
   Qed.
 End test6.
 
-Axiom admit : forall {T}, T.
+Axiom admit_pf : False.
+Notation admit := (match admit_pf with end).
+
+Ltac cache_reify _ :=
+  intros;
+  etransitivity;
+  [
+  | repeat apply (f_equal (fun f => f _));
+    Reify_rhs ();
+    reflexivity ];
+  cbv beta;
+  let RHS := match goal with |- _ = ?RHS => RHS end in
+  let e := match RHS with context[expr.Interp _ ?e] => e end in
+  let E := fresh "E" in
+  set (E := e);
+  let E' := constr:(PartialReduce (CPS.CallFunWithIdContinuation (CPS.Translate (canonicalize_list_recursion E)))) in
+  let LHS := match goal with |- ?LHS = _ => LHS end in
+  lazymatch LHS with
+  | context LHS[@expr.Interp ?ident ?interp_ident ?t ?e]
+    => let LHS := context LHS[@expr.Interp ident interp_ident t E'] in
+       transitivity LHS; [ | clear e ]
+  end;
+  [ repeat match goal with |- context[expr.Interp _ _ _] => apply (f_equal (fun f => f _)) end;
+    apply f_equal;
+    time lazy;
+    reflexivity
+  | clearbody E ].
 
 Derive carry_mul_gen
        SuchThat (forall (w : nat -> Z)
@@ -4977,31 +5364,117 @@ Derive carry_mul_gen
                            carry_mul_gen w s c n len_c idxs len_idxs fg
                     = carry_mulmod w s c n len_c idxs len_idxs fg)
        As carry_mul_gen_correct.
+Proof. Time cache_reify (). exact admit. (* correctness of initial parts of the pipeline *) Time Qed.
+
+Derive carry_gen
+       SuchThat (forall (w : nat -> Z)
+                        (f : list Z)
+                        (n : nat)
+                        (s : Z)
+                        (c : list (Z * Z))
+                        (len_c : nat)
+                        (idxs : list nat)
+                        (len_idxs : nat),
+                    Interp (t:=type.reify_type_of carrymod)
+                           carry_gen w s c n len_c idxs len_idxs f
+                    = carrymod w s c n len_c idxs len_idxs f)
+       As carry_gen_correct.
+Proof. cache_reify (). exact admit. (* correctness of initial parts of the pipeline *) Qed.
+
+Derive encode_gen
+       SuchThat (forall (w : nat -> Z)
+                        (v : Z)
+                        (n : nat)
+                        (s : Z)
+                        (c : list (Z * Z))
+                        (len_c : nat),
+                    Interp (t:=type.reify_type_of encodemod)
+                           encode_gen w s c n len_c v
+                    = encodemod w s c n len_c v)
+       As encode_gen_correct.
+Proof. cache_reify (). exact admit. (* correctness of initial parts of the pipeline *) Qed.
+
+Derive add_gen
+       SuchThat (forall (w : nat -> Z)
+                        (fg : list Z * list Z)
+                        (n : nat),
+                    Interp (t:=type.reify_type_of addmod)
+                           add_gen w n fg
+                    = addmod w n fg)
+       As add_gen_correct.
+Proof. cache_reify (). exact admit. (* correctness of initial parts of the pipeline *) Qed.
+
+Derive sub_gen
+       SuchThat (forall (w : nat -> Z)
+                        (n : nat)
+                        (s : Z)
+                        (c : list (Z * Z))
+                        (len_c : nat)
+                        (coef : Z)
+                        (fg : list Z * list Z),
+                    Interp (t:=type.reify_type_of submod)
+                           sub_gen w s c n len_c coef fg
+                    = submod w s c n len_c coef fg)
+       As sub_gen_correct.
+Proof. cache_reify (). exact admit. (* correctness of initial parts of the pipeline *) Qed.
+
+Derive opp_gen
+       SuchThat (forall (w : nat -> Z)
+                        (n : nat)
+                        (s : Z)
+                        (c : list (Z * Z))
+                        (len_c : nat)
+                        (coef : Z)
+                        (f : list Z),
+                    Interp (t:=type.reify_type_of oppmod)
+                           opp_gen w s c n len_c coef f
+                    = oppmod w s c n len_c coef f)
+       As opp_gen_correct.
+Proof. cache_reify (). exact admit. (* correctness of initial parts of the pipeline *) Qed.
+
+Definition zeromod w n s c len_c := encodemod w n s c len_c 0.
+Definition onemod w n s c len_c := encodemod w n s c len_c 1.
+
+Derive zero_gen
+       SuchThat (forall (w : nat -> Z)
+                        (n : nat)
+                        (s : Z)
+                        (c : list (Z * Z))
+                        (len_c : nat),
+                    Interp (t:=type.reify_type_of zeromod)
+                           zero_gen w s c n len_c
+                    = zeromod w s c n len_c)
+       As zero_gen_correct.
+Proof. cache_reify (). exact admit. (* correctness of initial parts of the pipeline *) Qed.
+
+Derive one_gen
+       SuchThat (forall (w : nat -> Z)
+                        (n : nat)
+                        (s : Z)
+                        (c : list (Z * Z))
+                        (len_c : nat),
+                    Interp (t:=type.reify_type_of onemod)
+                           one_gen w s c n len_c
+                    = onemod w s c n len_c)
+       As one_gen_correct.
+Proof. cache_reify (). exact admit. (* correctness of initial parts of the pipeline *) Qed.
+
+Definition expanding_id (n : nat) (ls : list Z) := expand_list (-1)%Z ls n.
+
+Lemma expanding_id_id n ls (H : List.length ls = n)
+  : expanding_id n ls = ls.
 Proof.
-  intros.
-  etransitivity.
-  Focus 2.
-  { repeat apply (f_equal (fun f => f _)).
-    Reify_rhs ().
-    reflexivity.
-  } Unfocus.
-  cbv beta.
-  let RHS := match goal with |- _ = ?RHS => RHS end in
-  let e := match RHS with context[expr.Interp _ ?e] => e end in
-  set (E := e).
-  Time let E' := constr:(PartialReduce (CPS.CallFunWithIdContinuation (CPS.Translate (canonicalize_list_recursion E)))) in
-       let E' := (eval vm_compute in E') in (* 0.131 for vm, about 0.6 for lazy, slower for native and cbv *)
-       pose E' as E''.
-  let LHS := match goal with |- ?LHS = _ => LHS end in
-  lazymatch LHS with
-  | context LHS[expr.Interp _ _]
-    => let LHS := context LHS[Interp E''] in
-       transitivity LHS
-  end;
-    [ clear E | exact admit ].
-  subst carry_mul_gen.
-  reflexivity.
+  unfold expanding_id. rewrite expand_list_correct by assumption; reflexivity.
 Qed.
+
+Derive id_gen
+       SuchThat (forall (n : nat)
+                        (ls : list Z),
+                    Interp (t:=type.reify_type_of expanding_id)
+                           id_gen n ls
+                    = expanding_id n ls)
+       As id_gen_correct.
+Proof. cache_reify (). exact admit. (* correctness of initial parts of the pipeline *) Qed.
 
 Module Pipeline.
   Inductive ErrorMessage :=
@@ -5010,6 +5483,7 @@ Module Pipeline.
   | Bounds_analysis_failed
   | Return_type_mismatch {T'} (found expected : T')
   | Value_not_le (descr : string) {T'} (lhs rhs : T')
+  | Value_not_lt (descr : string) {T'} (lhs rhs : T')
   | Values_not_provably_distinct (descr : string) {T'} (lhs rhs : T')
   | Values_not_provably_equal (descr : string) {T'} (lhs rhs : T').
 
@@ -5036,7 +5510,7 @@ Module Pipeline.
              arg_bounds
              out_bounds
              (E : Expr (s -> d))
-  : ErrorT (BoundsAnalysis.Indexed.expr.Notations.expr (BoundsAnalysis.AdjustBounds.ident.type_for_range relax_zrange (t:=BoundsAnalysis.Indexed.OfPHOAS.type.compile d) out_bounds))
+  : ErrorT (BoundsAnalysis.Indexed.expr.Notations.expr (BoundsAnalysis.Indexed.Range.type_for_range relax_zrange (t:=BoundsAnalysis.Indexed.OfPHOAS.type.compile d) out_bounds))
     := let E := PartialReduce E in
        let E := ReassociateSmallConstants.Reassociate (2^8) E in
        let E := BoundsAnalysis.OfPHOAS.AnalyzeBounds relax_zrange E arg_bounds in
@@ -5058,20 +5532,60 @@ Module Pipeline.
              rv
              (Hrv : BoundsPipeline relax_zrange arg_bounds out_bounds E = Success rv)
     : forall arg
+             (Harg : BoundsAnalysis.Indexed.Range.type_for_range_bounded_by
+                       relax_zrange
+                       arg_bounds arg = true)
              (arg' := @BoundsAnalysis.OfPHOAS.cast_back
                         s
                         relax_zrange
                         arg_bounds
                         arg),
-      BoundsAnalysis.OfPHOAS.Interp
-        (s:=s)
-        (d:=d)
-        relax_zrange
-        arg_bounds
-        (bs:=out_bounds)
-        arg
-        rv
-      = Some (Interp E arg').
+      exists res,
+        let ctx :=
+            BoundsAnalysis.Indexed.Context.extendb
+              (PositiveMap.empty _) 1 arg in
+        BoundsAnalysis.Indexed.expr.interp (@BoundsAnalysis.ident.interp) rv ctx
+        = Some res
+        /\ BoundsAnalysis.Indexed.Range.type_for_range_bounded_by
+             relax_zrange out_bounds res = true
+        /\ BoundsAnalysis.OfPHOAS.cast_back relax_zrange res
+           = Interp E arg'.
+  Proof.
+  Admitted.
+
+  Definition BoundsPipelineConst
+             relax_zrange
+             {t}
+             bounds
+             (E : Expr t)
+  : ErrorT (BoundsAnalysis.Indexed.expr.Notations.expr (BoundsAnalysis.Indexed.Range.type_for_range relax_zrange (t:=BoundsAnalysis.Indexed.OfPHOAS.type.compile t) bounds))
+    := let E := PartialReduce E in
+       let E := ReassociateSmallConstants.Reassociate (2^8) E in
+       let E := BoundsAnalysis.OfPHOAS.AnalyzeBoundsConst relax_zrange E in
+       let E := match E with
+                | Some (existT b v)
+                  => if BoundsAnalysis.Indexed.Range.range_is_tighter_than b bounds
+                     then transport_or_error BoundsAnalysis.Indexed.expr.Notations.expr v
+                     else Error (Computed_bounds_are_not_tight_enough b bounds)
+                | None => Error Bounds_analysis_failed
+                end in
+       E.
+
+  Lemma BoundsPipelineConst_correct
+             relax_zrange
+             {d}
+             bounds
+             (E : Expr d)
+             rv
+             (Hrv : BoundsPipelineConst relax_zrange bounds E = Success rv)
+    : exists res,
+        let ctx := PositiveMap.empty _ in
+        BoundsAnalysis.Indexed.expr.interp (@BoundsAnalysis.ident.interp) rv ctx
+        = Some res
+        /\ BoundsAnalysis.Indexed.Range.type_for_range_bounded_by
+             relax_zrange bounds res = true
+        /\ BoundsAnalysis.OfPHOAS.cast_back relax_zrange res
+           = Interp E.
   Proof.
   Admitted.
 End Pipeline.
@@ -5147,6 +5661,9 @@ Proof.
   reflexivity.
 Qed.
 
+Require Import Crypto.Algebra.Ring.
+Require Import Crypto.Arithmetic.PrimeFieldTheorems.
+
 (** XXX TODO: Translate Jade's python script *)
 Section rcarry_mul.
   Context (n : nat)
@@ -5156,7 +5673,12 @@ Section rcarry_mul.
 
   Let limbwidth := (Z.log2_up (s - Associational.eval c) / Z.of_nat n)%Q.
   Let idxs := (seq 0 n ++ [0; 1])%list%nat.
-  Let f_bounds := List.repeat r[0~>(2^Qceiling limbwidth + 2^(Qceiling limbwidth - 3))%Z]%zrange n.
+  Let upperbound_tight := (2^Qceiling limbwidth + 2^(Qceiling limbwidth - 3))%Z.
+  Let upperbound_loose := (3 * upperbound_tight)%Z.
+  Let f_bounds_tight := List.repeat r[0~>upperbound_tight]%zrange n.
+  Let f_bounds_loose := List.repeat r[0~>upperbound_loose]%zrange n.
+  Let prime_bound : BoundsAnalysis.Indexed.Range.range (BoundsAnalysis.Indexed.OfPHOAS.type.compile (type.Z))
+    := r[0~>(s - Associational.eval c - 1)]%zrange.
 
   Definition relax_zrange_of_machine_wordsize
     := relax_zrange_gen [machine_wordsize; 2 * machine_wordsize]%Z.
@@ -5169,23 +5691,30 @@ Section rcarry_mul.
   Let ridxs := GallinaReify.Reify idxs.
   Let rlen_c := GallinaReify.Reify (List.length c).
   Let rlen_idxs := GallinaReify.Reify (List.length idxs).
+  Let rcoef := GallinaReify.Reify 2.
   Let relax_zrange := relax_zrange_of_machine_wordsize.
-  Let arg_bounds : BoundsAnalysis.Indexed.Range.range (BoundsAnalysis.Indexed.OfPHOAS.type.compile (type.list type.Z * type.list type.Z))
-    := (f_bounds, f_bounds).
-  Let out_bounds : BoundsAnalysis.Indexed.Range.range (BoundsAnalysis.Indexed.OfPHOAS.type.compile (type.list type.Z))
-    := f_bounds.
+  Let tight_bounds : BoundsAnalysis.Indexed.Range.range (BoundsAnalysis.Indexed.OfPHOAS.type.compile (type.list type.Z))
+    := f_bounds_tight.
+  Let tight2_bounds : BoundsAnalysis.Indexed.Range.range (BoundsAnalysis.Indexed.OfPHOAS.type.compile (type.list type.Z * type.list type.Z))
+    := (tight_bounds, tight_bounds).
+  Let loose_bounds : BoundsAnalysis.Indexed.Range.range (BoundsAnalysis.Indexed.OfPHOAS.type.compile (type.list type.Z))
+    := f_bounds_loose.
+  Let loose2_bounds : BoundsAnalysis.Indexed.Range.range (BoundsAnalysis.Indexed.OfPHOAS.type.compile (type.list type.Z * type.list type.Z))
+    := (loose_bounds, loose_bounds).
 
   Definition check_args {T} (res : Pipeline.ErrorT T)
     : Pipeline.ErrorT T
     := if negb (Qle_bool 1 limbwidth)%Q
        then Pipeline.Error (Pipeline.Value_not_le "1 ≤ limbwidth" 1%Q limbwidth)
-       else if (s - Associational.eval c =? 0)%Z
-            then Pipeline.Error (Pipeline.Values_not_provably_distinct "s - Associational.eval c ≠ 0" (s - Associational.eval c) 0)
+       else if (negb (0 <? s - Associational.eval c))%Z
+            then Pipeline.Error (Pipeline.Value_not_lt "s - Associational.eval c ≤ 0" 0 (s - Associational.eval c))
             else if (s =? 0)%Z
                  then Pipeline.Error (Pipeline.Values_not_provably_distinct "s ≠ 0" s 0)
                  else if (n =? 0)%nat
                       then Pipeline.Error (Pipeline.Values_not_provably_distinct "n ≠ 0" n 0%nat)
-                      else res.
+                      else if (negb (0 <? machine_wordsize))
+                           then Pipeline.Error (Pipeline.Value_not_lt "0 < machine_wordsize" 0 machine_wordsize)
+                           else res.
 
   Lemma check_args_success_id {T} {rv : T} {res}
     : check_args res = Pipeline.Success rv
@@ -5194,13 +5723,114 @@ Section rcarry_mul.
     cbv [check_args]; break_innermost_match; congruence.
   Qed.
 
-  Definition rcarry_mul
+  Local Ltac solve_correct_gen pipeline_lem gen_correct :=
+    let Hrv := lazymatch goal with H : ?rop = Pipeline.Success _ |- _ => H end in
+    let rop := lazymatch type of Hrv with ?rop = Pipeline.Success _ => rop end in
+    hnf; intros; cbv [rop] in Hrv;
+    eapply pipeline_lem in Hrv; [ | eassumption.. ];
+    let res := fresh "res" in
+    destruct Hrv as [res Hrv];
+    exists res; do 2 try apply conj;
+    [ | | etransitivity ];
+    [ solve [ apply Hrv ].. | ];
+    repeat match goal with H := _ |- _ => subst H end;
+    erewrite <- gen_correct;
+    cbv [expr.Interp];
+    cbn [expr.interp];
+    f_equal;
+    cbn -[reify_list];
+    try (rewrite interp_reify_list, map_map; cbn;
+         erewrite map_ext with (g:=id), map_id; try reflexivity);
+    try (intros []; reflexivity).
+  Local Ltac solve_correct gen_correct :=
+    solve_correct_gen Pipeline.BoundsPipeline_correct gen_correct.
+  Local Ltac solve_correct_const gen_correct :=
+    solve_correct_gen Pipeline.BoundsPipelineConst_correct gen_correct.
+
+  Let BoundsPipeline21 in_bounds out_bounds res
     := let res := Pipeline.BoundsPipeline
-                    (relax_zrange)
+                    relax_zrange
                     (s:=(type.list type.Z * type.list type.Z)%ctype)
                     (d:=(type.list type.Z)%ctype)
-                    (arg_bounds)
-                    (out_bounds)
+                    (in_bounds, in_bounds)
+                    out_bounds
+                    res in
+       res.
+
+  Let BoundsPipeline11 in_bounds out_bounds res
+    := let res := Pipeline.BoundsPipeline
+                    relax_zrange
+                    (s:=(type.list type.Z)%ctype)
+                    (d:=(type.list type.Z)%ctype)
+                    (in_bounds)
+                    out_bounds
+                    res in
+       res.
+
+  Definition rexpr_1_correctT_ctx
+             ctx
+             out_bounds
+             (f : type.interp (type.list type.Z))
+             rv
+    := (exists res,
+           BoundsAnalysis.Indexed.expr.interp (@BoundsAnalysis.ident.interp) rv ctx
+           = Some res
+           /\ BoundsAnalysis.Indexed.Range.type_for_range_bounded_by
+                relax_zrange out_bounds res = true
+           /\ BoundsAnalysis.OfPHOAS.cast_back relax_zrange res
+              = f).
+
+  Definition rexpr_n1_correctT
+             t_in
+             in_bounds out_bounds
+             (f : _ -> type.interp (type.list type.Z))
+             rv
+    := forall arg
+              (arg' := @BoundsAnalysis.OfPHOAS.cast_back
+                         t_in
+                         relax_zrange
+                         in_bounds
+                         arg)
+              (Harg : BoundsAnalysis.Indexed.Range.type_for_range_bounded_by
+                        relax_zrange
+                        (t:=BoundsAnalysis.Indexed.OfPHOAS.type.compile t_in)
+                        in_bounds arg = true),
+      let ctx :=
+          BoundsAnalysis.Indexed.Context.extendb
+            (PositiveMap.empty _) 1 arg in
+      @rexpr_1_correctT_ctx ctx out_bounds (f arg') rv.
+
+  Definition rexpr_21_correctT
+             in_bounds out_bounds
+             (f : _ -> type.interp (type.list type.Z))
+             rv
+    := @rexpr_n1_correctT (type.list type.Z * type.list type.Z)
+                          (in_bounds, in_bounds) out_bounds f rv.
+
+  Definition rexpr_11_correctT
+             in_bounds out_bounds
+             (f : _ -> type.interp (type.list type.Z))
+             rv
+    := @rexpr_n1_correctT (type.list type.Z)
+                          in_bounds out_bounds f rv.
+
+  Definition rexpr_Z1_correctT
+             in_bounds out_bounds
+             (f : _ -> type.interp (type.list type.Z))
+             rv
+    := @rexpr_n1_correctT type.Z
+                          in_bounds out_bounds f rv.
+
+  Definition rexpr_01_correctT
+             out_bounds
+             (f : type.interp (type.list type.Z))
+             rv
+    := @rexpr_1_correctT_ctx (PositiveMap.empty _) out_bounds f rv.
+
+  Definition rcarry_mul
+    := let res := BoundsPipeline21
+                    loose_bounds
+                    tight_bounds
                     (fun var
                      => (carry_mul_gen _)
                           @ (rw _)
@@ -5211,84 +5841,733 @@ Section rcarry_mul.
                           @ (ridxs _)
                           @ (rlen_idxs _)
                     )%expr in
-       check_args res.
+       res.
 
   Definition rcarry_mul_correctT
              rv
-    := forall arg
-              (arg' := @BoundsAnalysis.OfPHOAS.cast_back
-                         _
-                         (relax_zrange)
-                         (arg_bounds)
-                         arg)
-              (Hf : List.length (fst arg) = n)
-              (Hg : List.length (snd arg) = n),
-      BoundsAnalysis.OfPHOAS.Interp
-        (relax_zrange)
-        (arg_bounds)
-        (bs:=out_bounds)
-        arg
-        rv
-      = Some (carry_mulmod (Interp rw) s c n (Interp rlen_c) idxs (Interp rlen_idxs) arg').
+    := Eval hnf in
+        rexpr_21_correctT
+          loose_bounds tight_bounds
+          (carry_mulmod (Interp rw) s c n (Interp rlen_c) idxs (Interp rlen_idxs))
+          rv.
 
   Lemma rcarry_mul_correct
-        rv
-        (Hrv : rcarry_mul = Pipeline.Success rv)
+        rv (Hrv : rcarry_mul = Pipeline.Success rv)
     : rcarry_mul_correctT rv.
-  Proof.
-    hnf; intros.
-    cbv [rcarry_mul] in Hrv.
-    edestruct (Pipeline.BoundsPipeline _ _ _ _) as [rv'|] eqn:Hrv';
-      [ | clear -Hrv; cbv [check_args] in Hrv; break_innermost_match_hyps; discriminate ].
-    erewrite <- carry_mul_gen_correct.
-    eapply Pipeline.BoundsPipeline_correct in Hrv'.
-    apply check_args_success_id in Hrv; inversion Hrv; subst rv.
-    rewrite Hrv'.
-    cbv [expr.Interp].
-    cbn [expr.interp].
-    apply f_equal; f_equal;
-      cbn -[reify_list];
-      rewrite interp_reify_list, map_map; cbn;
-        erewrite map_ext with (g:=id), map_id; try reflexivity.
-    intros []; reflexivity.
+  Proof. solve_correct carry_mul_gen_correct. Qed.
+
+  Definition rcarry
+    := let res := Pipeline.BoundsPipeline
+                    relax_zrange
+                    (s:=(type.list type.Z)%ctype)
+                    (d:=(type.list type.Z)%ctype)
+                    loose_bounds
+                    tight_bounds
+                    (fun var
+                     => (carry_gen _)
+                          @ (rw _)
+                          @ (rs _)
+                          @ (rc _)
+                          @ (rn _)
+                          @ (rlen_c _)
+                          @ (ridxs _)
+                          @ (rlen_idxs _)
+                    )%expr in
+       res.
+
+  Definition rcarry_correctT
+             rv
+    := Eval hnf in
+        rexpr_11_correctT
+          loose_bounds tight_bounds
+          (carrymod (Interp rw) s c n (Interp rlen_c) idxs (Interp rlen_idxs))
+          rv.
+
+  Lemma rcarry_correct
+        rv (Hrv : rcarry = Pipeline.Success rv)
+    : rcarry_correctT rv.
+  Proof. solve_correct carry_gen_correct. Qed.
+
+  Definition rrelax
+    := let res := Pipeline.BoundsPipeline
+                    relax_zrange
+                    (s:=(type.list type.Z)%ctype)
+                    (d:=(type.list type.Z)%ctype)
+                    tight_bounds
+                    loose_bounds
+                    (fun var
+                     => (id_gen _)
+                          @ (rn _)
+                    )%expr in
+       res.
+
+  Definition rrelax_correctT
+             rv
+    := Eval hnf in
+        rexpr_11_correctT
+          tight_bounds loose_bounds
+          (expanding_id n)
+          rv.
+
+  Lemma rrelax_correct
+        rv (Hrv : rrelax = Pipeline.Success rv)
+    : rrelax_correctT rv.
+  Proof. solve_correct id_gen_correct. Qed.
+
+  Definition radd
+    := let res := BoundsPipeline21
+                    tight_bounds
+                    loose_bounds
+                    (fun var
+                     => (add_gen _)
+                          @ (rw _)
+                          @ (rn _)
+                    )%expr in
+       res.
+
+  Definition radd_correctT
+             rv
+    := Eval hnf in
+        rexpr_21_correctT
+          tight_bounds loose_bounds
+          (addmod (Interp rw) n)
+          rv.
+
+  Lemma radd_correct
+        rv (Hrv : radd = Pipeline.Success rv)
+    : radd_correctT rv.
+  Proof. solve_correct add_gen_correct. Qed.
+
+  Definition rsub
+    := let res := BoundsPipeline21
+                    tight_bounds
+                    loose_bounds
+                    (fun var
+                     => (sub_gen _)
+                          @ (rw _)
+                          @ (rs _)
+                          @ (rc _)
+                          @ (rn _)
+                          @ (rlen_c _)
+                          @ (rcoef _)
+                    )%expr in
+       res.
+
+  Definition rsub_correctT
+             rv
+    := Eval hnf in
+        rexpr_21_correctT
+          tight_bounds loose_bounds
+          (submod (Interp rw) s c n (Interp rlen_c) (Interp rcoef))
+          rv.
+
+  Lemma rsub_correct
+        rv (Hrv : rsub = Pipeline.Success rv)
+    : rsub_correctT rv.
+  Proof. solve_correct sub_gen_correct. Qed.
+
+  Definition ropp
+    := let res := BoundsPipeline11
+                    tight_bounds
+                    loose_bounds
+                    (fun var
+                     => (opp_gen _)
+                          @ (rw _)
+                          @ (rs _)
+                          @ (rc _)
+                          @ (rn _)
+                          @ (rlen_c _)
+                          @ (rcoef _)
+                    )%expr in
+       res.
+
+  Definition ropp_correctT
+             rv
+    := Eval hnf in
+        rexpr_11_correctT
+          tight_bounds loose_bounds
+          (oppmod (Interp rw) s c n (Interp rlen_c) (Interp rcoef))
+          rv.
+
+  Lemma ropp_correct
+        rv (Hrv : ropp = Pipeline.Success rv)
+    : ropp_correctT rv.
+  Proof. solve_correct opp_gen_correct. Qed.
+
+  Definition rencode
+    := let res := Pipeline.BoundsPipeline
+                    relax_zrange
+                    (s:=type.Z)
+                    (d:=(type.list type.Z)%ctype)
+                    (prime_bound)
+                    tight_bounds
+                    (fun var
+                     => (encode_gen _)
+                          @ (rw _)
+                          @ (rs _)
+                          @ (rc _)
+                          @ (rn _)
+                          @ (rlen_c _)
+                    )%expr in
+       res.
+
+  Definition rencode_correctT
+             rv
+    := Eval hnf in
+        rexpr_Z1_correctT
+          prime_bound tight_bounds
+          (encodemod (Interp rw) s c n (Interp rlen_c))
+          rv.
+
+  Lemma rencode_correct
+        rv (Hrv : rencode = Pipeline.Success rv)
+    : rencode_correctT rv.
+  Proof. solve_correct encode_gen_correct. Qed.
+
+  Definition rzero
+    := let res := Pipeline.BoundsPipelineConst
+                    relax_zrange
+                    (t:=(type.list type.Z)%ctype)
+                    tight_bounds
+                    (fun var
+                     => (zero_gen _)
+                          @ (rw _)
+                          @ (rs _)
+                          @ (rc _)
+                          @ (rn _)
+                          @ (rlen_c _)
+                    )%expr in
+       res.
+
+  Definition rzero_correctT
+             rv
+    := Eval hnf in
+        rexpr_01_correctT
+          tight_bounds
+          (zeromod (Interp rw) s c n (Interp rlen_c))
+          rv.
+
+  Lemma rzero_correct
+        rv (Hrv : rzero = Pipeline.Success rv)
+    : rzero_correctT rv.
+  Proof. solve_correct_const zero_gen_correct. Qed.
+
+  Definition rone
+    := let res := Pipeline.BoundsPipelineConst
+                    relax_zrange
+                    (t:=(type.list type.Z)%ctype)
+                    tight_bounds
+                    (fun var
+                     => (one_gen _)
+                          @ (rw _)
+                          @ (rs _)
+                          @ (rc _)
+                          @ (rn _)
+                          @ (rlen_c _)
+                    )%expr in
+       res.
+
+  Definition rone_correctT
+             rv
+    := Eval hnf in
+        rexpr_01_correctT
+          tight_bounds
+          (onemod (Interp rw) s c n (Interp rlen_c))
+          rv.
+
+  Lemma rone_correct
+        rv (Hrv : rone = Pipeline.Success rv)
+    : rone_correctT rv.
+  Proof. solve_correct_const one_gen_correct. Qed.
+
+  Definition encodedT := { ls : option
+                                  (list (BoundsAnalysis.type.primitive.interp
+                                           (BoundsAnalysis.Indexed.Range.primitive_for_option_zrange
+                                              (relax_zrange (fold_right ZRange.union r[0 ~> 0]%zrange f_bounds_tight)))))
+                         |  exists res,
+                            ls = Some res
+                            /\ BoundsAnalysis.Indexed.Range.type_for_range_bounded_by
+                                 relax_zrange tight_bounds res = true }.
+
+  Program Definition list_of_encodedT (v : encodedT) : list _
+    := @Option.always_invert_Some
+         _
+         (proj1_sig v)
+         _.
+  Next Obligation.
+    repeat match goal with H : _ |- _ => clear H end.
+    destruct v as [? [? [H0 H1] ] ]; cbn; subst; congruence.
   Qed.
 
+  Lemma length_list_of_encodedT v : List.length (list_of_encodedT v) = n.
+  Proof.
+    destruct v as [v [res [Hpf H] ] ]; destruct v; cbn in *; [ | discriminate ].
+    apply BoundsAnalysis.Indexed.Range.length_list_bounded_by in H.
+    inversion_option; subst.
+    etransitivity; [ exact H | ].
+    subst tight_bounds f_bounds_tight.
+    rewrite repeat_length; reflexivity.
+  Qed.
 
-  (** This code may eventually be useful; it proves that [check_args]
-      is sufficient to satisfy the preconditions of
-      [eval_carry_mulmod] *)
-  (*
-<<
-    break_innermost_match_hyps; try solve [ exfalso; clear -Hrv; discriminate ]; [].
-    Z.ltb_to_lt.
-    rewrite negb_false_iff in *.
-    rewrite Qle_bool_iff in *.
-    rewrite NPeano.Nat.eqb_neq in *.
-    erewrite <- carry_mul_gen_correct
-      by (clear Hrv rv; try clear arg arg';
-          generalize (@pow_ceil_mul_nat_divide_nonzero 2 limbwidth);
-          generalize (@pow_ceil_mul_nat_nonzero 2 limbwidth);
-          cbv [Qceiling Qfloor Qopp Qnum Qdiv Qplus inject_Z Qmult Qinv Qden];
-          cbv [Qle] in *;
-          cbn; rewrite ?map_length, ?Z.mul_0_r, ?Pos.mul_1_r, ?Z.mul_1_r;
-          repeat match goal with H := _ |- _ => subst H || clear H end;
-          try destruct limbwidth; cbn in *;
-          do 2 try match goal with
-                   | [ |- forall _, _ ]
-                     => (let H := fresh in intro H; apply H) || intro
-                   end;
-          intros;
-          repeat match goal with
-                 | [ H : _ |- _ <> _ ] => eapply H
-                 end;
-          try reflexivity;
-          try lia).
->> *)
+  Let m : positive := Z.to_pos (s - Associational.eval c).
+  Definition Zdecode (v : encodedT)
+    := BoundsAnalysis.OfPHOAS.cast_back
+         (d:=type.list type.Z)
+         _
+         (list_of_encodedT v).
+  Definition Fdecode (v : encodedT) : F m
+    := F.of_Z m (Positional.eval (Interp rw) n (Zdecode v)).
+  Definition encodedT_eq (x y : encodedT)
+    := Fdecode x = Fdecode y.
+
+  Lemma length_Zdecode v : List.length (Zdecode v) = n.
+  Proof.
+    cbn [Zdecode BoundsAnalysis.OfPHOAS.cast_back].
+    rewrite map_length, length_list_of_encodedT; reflexivity.
+  Qed.
+
+  Section make_ring.
+    Context (curve_good : check_args (Pipeline.Success tt) = Pipeline.Success tt)
+            {rcarry_mulv} (Hrmulv : rcarry_mul_correctT rcarry_mulv)
+            {rcarryv} (Hrcarryv : rcarry_correctT rcarryv)
+            {rrelaxv} (Hrrelaxv : rrelax_correctT rrelaxv)
+            {raddv} (Hraddv : radd_correctT raddv)
+            {rsubv} (Hrsubv : rsub_correctT rsubv)
+            {roppv} (Hroppv : ropp_correctT roppv)
+            {rzerov} (Hrzerov : rzero_correctT rzerov)
+            {ronev} (Hronev : rone_correctT ronev)
+            {rencodev} (Hrencodev : rencode_correctT rencodev).
+
+    Local Ltac use_curve_good_t :=
+      repeat first [ progress rewrite ?map_length, ?Z.mul_0_r, ?Pos.mul_1_r, ?Z.mul_1_r in *
+                   | reflexivity
+                   | lia
+                   | rewrite interp_reify_list, ?map_map
+                   | rewrite map_ext with (g:=id), map_id
+                   | rewrite repeat_length
+                   | progress cbv [Qceiling Qfloor Qopp Qdiv Qplus inject_Z Qmult Qinv] in *
+                   | progress cbv [Qle] in *
+                   | progress cbn -[reify_list] in *
+                   | progress intros
+                   | solve [ auto ] ].
+
+    Lemma use_curve_good
+      : Z.pos m = s - Associational.eval c
+        /\ (Interp rw 0%nat = 1)
+        /\ (forall i, Interp rw i <> 0)
+        /\ ' m <> 0
+        /\ s - Associational.eval c <> 0
+        /\ s <> 0
+        /\ 0 < machine_wordsize
+        /\ n <> 0%nat
+        /\ List.length (Interp ridxs) = Interp rlen_idxs
+        /\ List.length (Interp rc) = Interp rlen_c
+        /\ List.length idxs = Interp rlen_idxs
+        /\ List.length c = Interp rlen_c
+        /\ List.length tight_bounds = n
+        /\ List.length loose_bounds = n
+        /\ forall i, Interp rw (S i) / Interp rw i <> 0.
+    Proof.
+      clear -curve_good.
+      cbv [check_args] in curve_good.
+      break_innermost_match_hyps; try discriminate.
+      rewrite negb_false_iff in *.
+      Z.ltb_to_lt.
+      rewrite Qle_bool_iff in *.
+      rewrite NPeano.Nat.eqb_neq in *.
+      generalize (@pow_ceil_mul_nat_divide_nonzero 2 limbwidth).
+      generalize (@pow_ceil_mul_nat_nonzero 2 limbwidth).
+      intros.
+      cbv [Qle] in *; cbn [Qnum Qden] in *.
+      cbv [Qceiling Qfloor Qopp Qdiv Qplus inject_Z Qmult Qinv] in *.
+      cbn [Qnum Qden] in *.
+      rewrite ?map_length, ?Z.mul_0_r, ?Pos.mul_1_r, ?Z.mul_1_r in *.
+      specialize_by lia.
+      repeat match goal with H := _ |- _ => subst H end.
+      repeat apply conj.
+      { destruct (s - Associational.eval c); cbn; lia. }
+      { use_curve_good_t. }
+      { use_curve_good_t. }
+      { use_curve_good_t. }
+      { use_curve_good_t. }
+      { use_curve_good_t. }
+      { use_curve_good_t. }
+      { use_curve_good_t. }
+      { use_curve_good_t. }
+      { use_curve_good_t. }
+      { use_curve_good_t. }
+      { use_curve_good_t. }
+      { use_curve_good_t. }
+      { use_curve_good_t. }
+      { use_curve_good_t. }
+    Qed.
+
+    Local Lemma m_eq : Z.pos m = s - Associational.eval c.
+    Proof. apply use_curve_good. Qed.
+
+    Local Lemma sc_pos : 0 < s - Associational.eval c.
+    Proof. pose proof use_curve_good; destruct_head'_and; lia. Qed.
+
+    Local Lemma length_tight_bounds : List.length tight_bounds = n.
+    Proof. apply use_curve_good. Qed.
+
+    Local Lemma length_loose_bounds : List.length loose_bounds = n.
+    Proof. apply use_curve_good. Qed.
+
+    Local Arguments Z.pow !_ !_ .
+    Lemma relax_is_good
+      : BoundsAnalysis.OfPHOAS.relax_is_good relax_zrange.
+    Proof.
+      cbn; cbv [BoundsAnalysis.OfPHOAS.relax_is_good relax_zrange_gen]; cbn.
+      intros [l u] [l' u']; cbn.
+      pose proof (Z.log2_up_nonneg (u + 1)).
+      destruct (Z.log2_up_null (u + 1)).
+      unfold is_tighter_than_bool; rewrite Bool.andb_true_iff;
+        break_innermost_match; cbn; Z.ltb_to_lt; intros;
+          inversion_option; inversion_zrange; subst;
+            repeat apply conj; Z.ltb_to_lt; try omega;
+              try (rewrite <- ZUtil.Z.log2_up_le_pow2_full in * by lia; cbn in *; lia).
+    Qed.
+
+    Local Notation option_interp0 f
+      := (BoundsAnalysis.Indexed.expr.interp
+            (@BoundsAnalysis.ident.interp)
+            f
+            (PositiveMap.empty _)).
+
+    Local Notation option_interp1 f arg
+      := (arg' <- arg;
+            BoundsAnalysis.Indexed.expr.interp
+              (@BoundsAnalysis.ident.interp)
+              f
+              (BoundsAnalysis.Indexed.Context.extendb
+                 (T:=BoundsAnalysis.type.list _)
+                 (PositiveMap.empty _)
+                 1 arg'))%option.
+
+    Local Notation option_interp2 f arg1 arg2
+      := (x <- arg1;
+            y <- arg2;
+            BoundsAnalysis.Indexed.expr.interp
+              (@BoundsAnalysis.ident.interp)
+              f
+              (BoundsAnalysis.Indexed.Context.extendb
+                 (T:=BoundsAnalysis.type.prod
+                       (BoundsAnalysis.type.list _)
+                       (BoundsAnalysis.type.list _))
+                 (PositiveMap.empty _)
+                 1 (x, y)))%option.
+
+    Local Ltac solve_encodedT _ :=
+      repeat match goal with
+             | _ => progress destruct_head' encodedT
+             | _ => progress (destruct_head'_ex; destruct_head'_and; subst)
+             | _ => progress cbn [proj1_sig Option.bind always_invert_Some] in *
+             | [ H : ?x = Some _ |- context[?x] ] => rewrite H
+             | [ H : ?x = Some _, H' : context[?x] |- _ ] => rewrite H in H'
+             | [ |- BoundsAnalysis.Indexed.Range.type_for_range_bounded_by _ _ (_, _) = true ]
+               => progress cbn [BoundsAnalysis.Indexed.Range.type_for_range_bounded_by BoundsAnalysis.Indexed.OfPHOAS.type.compile]
+             | _ => progress cbn [BoundsAnalysis.Indexed.Range.type_for_range BoundsAnalysis.Indexed.OfPHOAS.type.compile fst snd] in * (* for getting rewrite to match *)
+             | [ |- andb _ _ = true ] => rewrite Bool.andb_true_iff
+             | _ => solve [ eauto ]
+             | [ |- sig _ ] => progress rewrite expanding_id_id in *
+             | [ |- List.length (List.map _ _) = _ ] => rewrite map_length
+             | [ H : BoundsAnalysis.Indexed.Range.type_for_range_bounded_by _ _ ?x = true
+                 |- List.length ?x = _ ]
+               => erewrite BoundsAnalysis.Indexed.Range.length_list_bounded_by by exact H
+             | _ => progress rewrite ?length_tight_bounds, ?length_loose_bounds
+             | [ H : map _ ?x = map _ _ |- _ ] => rewrite H in *
+             | [ H : map _ ?x = _ |- context[map _ ?x] ]
+               => cbv [tight_bounds loose_bounds] in H |- *; rewrite H
+             | _ => rewrite BoundsAnalysis.OfPHOAS.cast_back_primitive_cast_primitive in *
+             | [ fx := (BoundsAnalysis.Indexed.expr.interp _ ?rop (BoundsAnalysis.Indexed.Context.extendb _ _ ?x)),
+                       H : forall arg, BoundsAnalysis.Indexed.Range.type_for_range_bounded_by _ ?bs arg = true -> rexpr_1_correctT_ctx _ _ _ ?rop
+                                       |- _ ]
+               => destruct (H x); [ clear H | subst fx ]
+             | [ fx := Option.bind ?x ?f, H : ?x = Some ?v |- _ ]
+               => let H' := fresh in
+                  let fx' := fresh fx in
+                  pose (Option.bind (Some v) f) as fx';
+                  assert (H' : fx = fx')
+                    by (subst fx fx'; apply f_equal2; [ exact H | reflexivity ]);
+                  cbn [Option.bind] in fx'; clearbody fx; subst fx
+             (*| [ H : forall arg, BoundsAnalysis.Indexed.Range.type_for_range_bounded_by _ ?bs arg = true -> rexpr_1_correctT_ctx _ _ _ ?rop
+                                 |- context[BoundsAnalysis.Indexed.expr.interp _ ?rop (BoundsAnalysis.Indexed.Context.extendb _ _ ?x)] ]
+               => specialize (H x); destruct H*)
+             | _ => progress cbn [BoundsAnalysis.OfPHOAS.cast_back] in * (* for getting eauto to work *)
+             end.
+
+    Definition ring_mul_sig
+      : forall (x y : encodedT),
+        { v : encodedT
+        | Zdecode v = carry_mulmod (Interp rw) s c n (Interp rlen_c) idxs (Interp rlen_idxs) (Zdecode x, Zdecode y) }.
+    Proof.
+      simple refine
+             (fun x y
+              => let x' := option_interp1 rrelaxv (proj1_sig x) in
+                 let y' := option_interp1 rrelaxv (proj1_sig y) in
+                 let v' := option_interp2 rcarry_mulv x' y' in
+                 let pf : { pf0 : _ | Zdecode (exist _ v' pf0) = _ }
+                     := _ in
+                 exist _ (exist _ v' (proj1_sig pf)) (proj2_sig pf)).
+      cbv [Zdecode list_of_encodedT]; cbn [proj1_sig].
+      hnf in Hrrelaxv, Hrmulv.
+      abstract solve_encodedT ().
+    Defined.
+
+    Definition ring_add_sig
+      : forall (x y : encodedT),
+        { v : encodedT
+        | Zdecode v = carrymod
+                        (Interp rw) s c n (Interp rlen_c) idxs (Interp rlen_idxs)
+                        (addmod (Interp rw) n (Zdecode x, Zdecode y)) }.
+    Proof.
+      simple refine
+             (fun x y
+              => let v'' := option_interp2 raddv (proj1_sig x) (proj1_sig y) in
+                 let v' := option_interp1 rcarryv v'' in
+                 let pf : { pf0 : _ | Zdecode (exist _ v' pf0) = _ }
+                     := _ in
+                 exist _ (exist _ v' (proj1_sig pf)) (proj2_sig pf)).
+      cbv [Zdecode list_of_encodedT]; cbn [proj1_sig].
+      hnf in Hrcarryv, Hraddv; clear -Hrcarryv Hraddv.
+      abstract solve_encodedT ().
+    Defined.
+    Definition ring_sub_sig
+      : forall (x y : encodedT),
+        { v : encodedT
+        | Zdecode v = carrymod
+                        (Interp rw) s c n (Interp rlen_c) idxs (Interp rlen_idxs)
+                        (submod (Interp rw) s c n (Interp rlen_c) (Interp rcoef) (Zdecode x, Zdecode y)) }.
+    Proof.
+      simple refine
+             (fun x y
+              => let v'' := option_interp2 rsubv (proj1_sig x) (proj1_sig y) in
+                 let v' := option_interp1 rcarryv v'' in
+                 let pf : { pf0 : _ | Zdecode (exist _ v' pf0) = _ }
+                     := _ in
+                 exist _ (exist _ v' (proj1_sig pf)) (proj2_sig pf)).
+      cbv [Zdecode list_of_encodedT]; cbn [proj1_sig].
+      hnf in Hrcarryv, Hrsubv.
+      abstract solve_encodedT ().
+    Defined.
+    Definition ring_opp_sig
+      : forall (x : encodedT),
+        { v : encodedT
+        | Zdecode v = carrymod
+                        (Interp rw) s c n (Interp rlen_c) idxs (Interp rlen_idxs)
+                        (oppmod (Interp rw) s c n (Interp rlen_c) (Interp rcoef) (Zdecode x)) }.
+    Proof.
+      simple refine
+             (fun x
+              => let v'' := option_interp1 roppv (proj1_sig x) in
+                 let v' := option_interp1 rcarryv v'' in
+                 let pf : { pf0 : _ | Zdecode (exist _ v' pf0) = _ }
+                     := _ in
+                 exist _ (exist _ v' (proj1_sig pf)) (proj2_sig pf)).
+      cbv [Zdecode list_of_encodedT]; cbn [proj1_sig].
+      hnf in Hrcarryv, Hroppv.
+      abstract solve_encodedT ().
+    Defined.
+    Definition ring_zero_sig
+      : { v : encodedT
+        | Zdecode v = zeromod
+                        (Interp rw) s c n (Interp rlen_c) }.
+    Proof.
+      simple refine
+             (let v' := option_interp0 rzerov in
+              let pf : { pf0 : _ | Zdecode (exist _ v' pf0) = _ }
+                  := _ in
+              exist _ (exist _ v' (proj1_sig pf)) (proj2_sig pf)).
+      cbv [Zdecode list_of_encodedT]; cbn [proj1_sig].
+      abstract (
+          destruct Hrzerov; subst v';
+          solve_encodedT ()
+        ).
+    Defined.
+    Definition ring_one_sig
+      : { v : encodedT
+        | Zdecode v = onemod
+                        (Interp rw) s c n (Interp rlen_c) }.
+    Proof.
+      simple refine
+             (let v' := option_interp0 ronev in
+              let pf : { pf0 : _ | Zdecode (exist _ v' pf0) = _ }
+                  := _ in
+              exist _ (exist _ v' (proj1_sig pf)) (proj2_sig pf)).
+      cbv [Zdecode list_of_encodedT]; cbn [proj1_sig].
+      abstract (
+          destruct Hronev; subst v';
+          solve_encodedT ()
+        ).
+    Defined.
+    Arguments Z.mul !_ !_ .
+    Definition ring_encode_sig
+      : forall (x : F m),
+        { v : encodedT
+        | Zdecode v = encodemod
+                        (Interp rw) s c n (Interp rlen_c) (F.to_Z x) }.
+    Proof.
+      simple refine
+             (fun v
+              => let pf0 := _ in
+                 let pf1 := _ in
+                 let arg := BoundsAnalysis.OfPHOAS.cast_primitiveZ
+                              relax_zrange
+                              (F.to_Z v) relax_is_good pf0 in
+                 let Hrencodev' := Hrencodev arg pf1 in
+                 let v' := BoundsAnalysis.Indexed.expr.interp
+                             (@BoundsAnalysis.ident.interp)
+                             rencodev
+                             (BoundsAnalysis.Indexed.Context.extendb
+                                (T:=BoundsAnalysis.type.type_primitive _)
+                                (PositiveMap.empty _)
+                                1 arg) in
+                 let pf : { pf0 : _ | Zdecode (exist _ v' pf0) = _ }
+                     := _ in
+                 exist _ (exist _ v' (proj1_sig pf)) (proj2_sig pf)).
+      { pose proof use_curve_good as keep.
+        clear -curve_good keep.
+        abstract (
+            split; [ | exact I ];
+            destruct v as [v Hv]; hnf; cbn;
+            rewrite m_eq in Hv; rewrite Hv;
+            pose proof (Z.mod_pos_bound v _ sc_pos); lia
+          ). }
+      { clearbody pf0.
+        clear -pf0.
+        cbn.
+        (** TODO: clean up this part of the proof.  It is annoying
+            because [BoundsAnalysis.OfPHOAS.cast_primitiveZ] and
+            [BoundsAnalysis.Indexed.Range.type_for_range_bounded_by]
+            use different notions of the "interpretation" of a
+            not-necessarily-Z thing as probably-a-Z *)
+        generalize (BoundsAnalysis.OfPHOAS.cast_back_primitive_cast_primitive
+                      relax_zrange _ _ relax_is_good pf0).
+        generalize (BoundsAnalysis.OfPHOAS.cast_primitiveZ
+                      relax_zrange (F.to_Z v) relax_is_good pf0).
+        generalize (relax_is_good prime_bound).
+        cbv [BoundsAnalysis.Indexed.Range.primitive_bounded_by].
+        cbn [BoundsAnalysis.type.primitive.interp].
+        cbv [BoundsAnalysis.OfPHOAS.cast_back_primitive].
+        cbv [BoundsAnalysis.Indexed.Range.primitive_for_zrange].
+        abstract (
+            break_innermost_match; cbn;
+            intros; destruct_head' BoundsAnalysis.type.BoundedZ; cbn [BoundsAnalysis.type.value] in *;
+            subst;
+            hnf in pf0;
+            cbv [prime_bound is_tighter_than_bool] in *;
+            try lazymatch goal with
+                | [ H : forall _, Some _ = Some _ -> _ |- _ ]
+                  => specialize (H _ eq_refl)
+                end;
+            rewrite ?Bool.andb_true_iff in *;
+            destruct_head'_and;
+            apply conj; Z.ltb_to_lt;
+            cbn [upper lower] in *;
+            try omega
+          ). }
+      { cbv [Zdecode list_of_encodedT]; cbn [proj1_sig].
+        subst v' arg; clearbody Hrencodev'; cbv beta zeta in *.
+        abstract (
+            destruct Hrencodev';
+            solve_encodedT ()
+          ). }
+    Defined.
+
+    Lemma length_addmod x y
+      : List.length (addmod (Interp rw) n (Zdecode x, Zdecode y)) = n.
+    Proof.
+      cbv [addmod]; apply length_add; rewrite expand_list_correct;
+        cbn [fst snd]; apply length_Zdecode.
+    Qed.
+    Lemma length_submod x y
+      : List.length (submod (Interp rw) s c n (Interp rlen_c) (Interp rcoef) (Zdecode x, Zdecode y)) = n.
+    Proof.
+      cbv [submod]; apply length_sub; rewrite expand_list_correct;
+        cbn [fst snd]; apply length_Zdecode.
+    Qed.
+    Lemma length_oppmod x
+      : List.length (oppmod (Interp rw) s c n (Interp rlen_c) (Interp rcoef) (Zdecode x)) = n.
+    Proof.
+      cbv [oppmod]; apply length_opp; rewrite expand_list_correct;
+        cbn [fst snd]; apply length_Zdecode.
+    Qed.
+
+    Definition ring_mul x y := proj1_sig (ring_mul_sig x y).
+    Definition ring_add x y := proj1_sig (ring_add_sig x y).
+    Definition ring_sub x y := proj1_sig (ring_sub_sig x y).
+    Definition ring_opp x := proj1_sig (ring_opp_sig x).
+    Definition ring_zero := proj1_sig ring_zero_sig.
+    Definition ring_one := proj1_sig ring_one_sig.
+    Definition ring_encode x := proj1_sig (ring_encode_sig x).
+
+    Definition GoodT : Prop
+      := @Hierarchy.ring
+           encodedT encodedT_eq ring_zero ring_one ring_opp ring_add ring_sub ring_mul
+         /\ @Ring.is_homomorphism
+              (F m) eq 1%F F.add F.mul
+              encodedT encodedT_eq ring_one ring_add ring_mul ring_encode
+         /\ @Ring.is_homomorphism
+              encodedT encodedT_eq ring_one ring_add ring_mul
+              (F m) eq 1%F F.add F.mul
+              Fdecode.
+
+    Hint Rewrite ->@F.to_Z_add : push_FtoZ.
+    Hint Rewrite ->@F.to_Z_mul : push_FtoZ.
+    Hint Rewrite ->@F.to_Z_opp : push_FtoZ.
+    Hint Rewrite ->@F.to_Z_of_Z : push_FtoZ.
+
+    Local Ltac rewrite_proj2_sig _ :=
+      lazymatch goal with
+      | [ |- context[proj1_sig ?x] ] => rewrite (proj2_sig x)
+      end.
+
+    Lemma Good : GoodT.
+    Proof.
+      pose proof use_curve_good.
+      destruct_head'_and.
+      eapply ring_by_isomorphism; intros; [ | reflexivity | .. ]; rewrite F.eq_to_Z_iff;
+        cbv [F.sub Fdecode];
+        autorewrite with push_FtoZ;
+        pull_Zmod;
+        rewrite ?Z.add_opp_r.
+      { cbv [ring_encode]; rewrite_proj2_sig ().
+        erewrite m_eq, eval_encodemod, <- m_eq by assumption.
+        let A := lazymatch goal with A : F _ |- _ => A end in
+        destruct A as [v Hv]; cbn; congruence. }
+      { cbv [ring_zero]; rewrite_proj2_sig ().
+        cbv [zeromod]; erewrite m_eq, eval_encodemod, Zmod_0_l by eassumption; reflexivity. }
+      { cbv [ring_one]; rewrite_proj2_sig ().
+        cbv [onemod]; cbn; erewrite m_eq, eval_encodemod by eassumption; reflexivity. }
+      { cbv [ring_opp]; rewrite_proj2_sig ().
+        erewrite m_eq, eval_carrymod, eval_oppmod
+          by eauto using length_Zdecode, length_oppmod;
+          reflexivity. }
+      { cbv [ring_add]; rewrite_proj2_sig ().
+        erewrite m_eq, eval_carrymod, eval_addmod
+          by eauto using length_Zdecode, length_addmod;
+          reflexivity. }
+      { cbv [ring_sub]; rewrite_proj2_sig ().
+        erewrite m_eq, eval_carrymod, eval_submod
+          by eauto using length_Zdecode, length_submod;
+          reflexivity. }
+      { cbv [ring_mul]; rewrite_proj2_sig ().
+        erewrite m_eq, eval_carry_mulmod
+          by eauto using length_Zdecode; reflexivity. }
+    Qed.
+  End make_ring.
 End rcarry_mul.
 
-Ltac solve_rcarry_mul _ :=
-  eapply rcarry_mul_correct;
-  lazy; reflexivity.
+Ltac solve_rcarry_mul _ := eapply rcarry_mul_correct; lazy; reflexivity.
+Ltac solve_rcarry _ := eapply rcarry_correct; lazy; reflexivity.
+Ltac solve_radd _ := eapply radd_correct; lazy; reflexivity.
+Ltac solve_rsub _ := eapply rsub_correct; lazy; reflexivity.
+Ltac solve_ropp _ := eapply ropp_correct; lazy; reflexivity.
+Ltac solve_rencode _ := eapply rencode_correct; lazy; reflexivity.
+Ltac solve_rrelax _ := eapply rrelax_correct; lazy; reflexivity.
+Ltac solve_rzero _ := eapply rzero_correct; lazy; reflexivity.
+Ltac solve_rone _ := eapply rone_correct; lazy; reflexivity.
 
 Module PrintingNotations.
   Export ident.
@@ -5303,6 +6582,8 @@ Module PrintingNotations.
     := (r[0 ~> 18446744073709551615]) : btype_scope.
   Notation "'uint32'"
     := (r[0 ~> 4294967295]) : btype_scope.
+  Notation "'ℤ'"
+    := BoundsAnalysis.type.Z : btype_scope.
   Notation "ls [[ n ]]" := (List.nth n @@ ls)%nexpr : nexpr_scope.
   Notation "x *₆₄₋₆₄₋₁₂₈ y"
     := (mul uint64 uint64 uint128 @@ (x, y))%nexpr (at level 40) : nexpr_scope.
@@ -5326,6 +6607,16 @@ Module PrintingNotations.
     := (add uint64 uint64 uint64 @@ (x, y))%nexpr (at level 50) : nexpr_scope.
   Notation "x +₃₂ y"
     := (add uint32 uint32 uint32 @@ (x, y))%nexpr (at level 50) : nexpr_scope.
+  Notation "x -₁₂₈ y"
+    := (sub uint128 uint128 uint128 @@ (x, y))%nexpr (at level 50) : nexpr_scope.
+  Notation "x -₆₄₋₁₂₈₋₁₂₈ y"
+    := (sub uint64 uint128 uint128 @@ (x, y))%nexpr (at level 50) : nexpr_scope.
+  Notation "x -₃₂₋₆₄₋₆₄ y"
+    := (sub uint32 uint64 uint64 @@ (x, y))%nexpr (at level 50) : nexpr_scope.
+  Notation "x -₆₄ y"
+    := (sub uint64 uint64 uint64 @@ (x, y))%nexpr (at level 50) : nexpr_scope.
+  Notation "x -₃₂ y"
+    := (sub uint32 uint32 uint32 @@ (x, y))%nexpr (at level 50) : nexpr_scope.
   Notation "x" := ({| BoundsAnalysis.type.value := x |}) (only printing) : nexpr_scope.
   Notation "( out_t )( v >> count )"
     := ((shiftr _ out_t count @@ v)%nexpr)
@@ -5363,6 +6654,58 @@ Module X25519_64.
          SuchThat (rcarry_mul_correctT n s c machine_wordsize base_51_carry_mul)
          As base_51_carry_mul_correct.
   Proof. Time solve_rcarry_mul (). Time Qed.
+  Derive base_51_carry
+         SuchThat (rcarry_correctT n s c machine_wordsize base_51_carry)
+         As base_51_carry_correct.
+  Proof. Time solve_rcarry (). Time Qed.
+  Derive base_51_relax
+         SuchThat (rrelax_correctT n s c machine_wordsize base_51_relax)
+         As base_51_relax_correct.
+  Proof. Time solve_rrelax (). Time Qed.
+  Derive base_51_add
+         SuchThat (radd_correctT n s c machine_wordsize base_51_add)
+         As base_51_add_correct.
+  Proof. Time solve_radd (). Time Qed.
+  Derive base_51_sub
+         SuchThat (rsub_correctT n s c machine_wordsize base_51_sub)
+         As base_51_sub_correct.
+  Proof. Time solve_rsub (). Time Qed.
+  Derive base_51_opp
+         SuchThat (ropp_correctT n s c machine_wordsize base_51_opp)
+         As base_51_opp_correct.
+  Proof. Time solve_ropp (). Time Qed.
+  Derive base_51_encode
+         SuchThat (rencode_correctT n s c machine_wordsize base_51_encode)
+         As base_51_encode_correct.
+  Proof. Time solve_rencode (). Time Qed.
+  Derive base_51_zero
+         SuchThat (rzero_correctT n s c machine_wordsize base_51_zero)
+         As base_51_zero_correct.
+  Proof. Time solve_rzero (). Time Qed.
+  Derive base_51_one
+         SuchThat (rone_correctT n s c machine_wordsize base_51_one)
+         As base_51_one_correct.
+  Proof. Time solve_rone (). Time Qed.
+  Lemma base_51_curve_good
+    : check_args n s c machine_wordsize (Pipeline.Success tt) = Pipeline.Success tt.
+  Proof. vm_compute; reflexivity. Qed.
+
+  Definition base_51_goodT
+    := GoodT n s c machine_wordsize
+             base_51_curve_good
+             base_51_carry_mul_correct
+             base_51_carry_correct
+             base_51_relax_correct
+             base_51_add_correct
+             base_51_sub_correct
+             base_51_opp_correct
+             base_51_zero_correct
+             base_51_one_correct
+             base_51_encode_correct.
+  Theorem base_51_good : base_51_goodT.
+  Proof. apply Good. Qed.
+
+  Print Assumptions base_51_good.
 
   Import PrintingNotations.
   Print base_51_carry_mul.
@@ -5415,8 +6758,16 @@ Module X25519_64.
  x_19 :: x_22 :: x_21 +₆₄ x_10 :: x_13 :: x_16 :: [])%nexpr
      : expr
          (BoundsAnalysis.AdjustBounds.ident.type_for_range
-            (relax_zrange (make_carry_mul_rargs limbwidth s c machine_wordsize))
-            (out_bounds (make_carry_mul_rargs limbwidth s c machine_wordsize)))
+            (relax_zrange_of_machine_wordsize machine_wordsize)
+            (List.repeat
+               r[0 ~> 2
+                      ^ Qceiling
+                          (inject_Z (Z.log2_up (s - Associational.eval c)) /
+                           inject_Z (BinInt.Z.of_nat n)) +
+                      2
+                      ^ (Qceiling
+                           (inject_Z (Z.log2_up (s - Associational.eval c)) /
+                            inject_Z (BinInt.Z.of_nat n)) - 3)]%zrange n))
 *)
 End X25519_64.
 
@@ -5593,8 +6944,8 @@ Module X25519_32.
  x_34 :: x_37 :: x_36 +₃₂ x_10 :: x_13 :: x_16 :: x_19 :: x_22 :: x_25 :: x_28 :: x_31 :: [])%nexpr
      : expr
          (BoundsAnalysis.AdjustBounds.ident.type_for_range
-            (relax_zrange (make_carry_mul_rargs limbwidth s c machine_wordsize))
-            (out_bounds (make_carry_mul_rargs limbwidth s c machine_wordsize)))
+            (relax_zrange (make_carry_mul_rargs n s c machine_wordsize))
+            (out_bounds (make_carry_mul_rargs n s c machine_wordsize)))
 *)
 End X25519_32.
 *)
